ft_tests/Timeout.bpl
@@ -10,10 +10,8 @@ type State;
 var M: MType;
 var C: CType;
 var R: CType;
-var L: CType;
+var I: CType;
 var St: [Actor]State;
-const Base#L: int;
-axiom 1 <= Base#L;
 
 const unique this#: Actor;
 type List a = [int]a;
@@ -29,61 +27,55 @@ var SqnAct: [Actor]int;
 // -- End of prelude ---------------------------------------------
 // ---------------------------------------------------------------
 
-axiom Base#L == 1;
 procedure Rep#anon$0#0()
-  modifies C, R, M, St, SqnCh, SqnAct;
+  modifies C, R, M, I, St, SqnCh, SqnAct;
 {
   var in: Chan (int);
   var out: Chan (int);
   assume true;
-  assume true;
 }
 procedure Split#anon$1#1()
-  modifies C, R, M, St, SqnCh, SqnAct;
+  modifies C, R, M, I, St, SqnCh, SqnAct;
 {
   var in: Chan (int);
   var out1: Chan (int);
   var out2: Chan (int);
   assume true;
-  assume true;
 }
 procedure Adjudicator#normal#2()
-  modifies C, R, M, St, SqnCh, SqnAct;
+  modifies C, R, M, I, St, SqnCh, SqnAct;
 {
   var x1: Chan (int);
   var x2: Chan (int);
   var c_in: Chan (int);
   var y: Chan (int);
   var c_out: Chan (int);
-  assume true;
   assume (SqnCh[x1][0] == SqnCh[x2][0]) && (SqnCh[x1][0] == M[c_in][0]);
   assume true;
 }
 procedure Adjudicator#timeout#3()
-  modifies C, R, M, St, SqnCh, SqnAct;
+  modifies C, R, M, I, St, SqnCh, SqnAct;
 {
   var x1: Chan (int);
   var x2: Chan (int);
   var c_in: Chan (int);
   var y: Chan (int);
   var c_out: Chan (int);
-  assume true;
   assume true;
 }
 procedure Adjudicator#readoff#4()
-  modifies C, R, M, St, SqnCh, SqnAct;
+  modifies C, R, M, I, St, SqnCh, SqnAct;
 {
   var x1: Chan (int);
   var x2: Chan (int);
   var c_in: Chan (int);
   var y: Chan (int);
   var c_out: Chan (int);
-  assume true;
   assume SqnCh[x1][0] < M[c_in][0];
   assume true;
 }
 procedure Adjudicator#anon$2#5()
-  modifies C, R, M, St, SqnCh, SqnAct;
+  modifies C, R, M, I, St, SqnCh, SqnAct;
 {
   var x1: Chan (int);
   var x2: Chan (int);
@@ -91,11 +83,55 @@ procedure Adjudicator#anon$2#5()
   var y: Chan (int);
   var c_out: Chan (int);
   assume true;
-  assume true;
 }
-procedure Net#init#6()
-  modifies C, R, M, St, SqnCh, SqnAct;
+procedure Adjudicator##GuardWD#6()
+  modifies C, R, M, I, St, SqnCh, SqnAct;
 {
+  var x2: Chan (int);
+  var c_in: Chan (int);
+  var y: Chan (int);
+  var c_out: Chan (int);
+  var x1: Chan (int);
+  assert {:msg "12.1: The actions of actor 'Adjudicator' might not have mutually exclusive guards (#0)"} !((1 <= (C[x1] - R[x1])) && (1 <= (C[x2] - R[x2])) && (1 <= (C[c_in] - R[c_in])) && (SqnCh[x1][0] == SqnCh[x2][0]) && (SqnCh[x1][0] == M[c_in][0]) && (1 <= (C[x2] - R[x2])) && (1 <= (C[c_in] - R[c_in])));
+  assert {:msg "12.1: The actions of actor 'Adjudicator' might not have mutually exclusive guards (#1)"} !((1 <= (C[x1] - R[x1])) && (1 <= (C[x2] - R[x2])) && (1 <= (C[c_in] - R[c_in])) && (SqnCh[x1][0] == SqnCh[x2][0]) && (SqnCh[x1][0] == M[c_in][0]) && (1 <= (C[x1] - R[x1])) && (1 <= (C[c_in] - R[c_in])) && (SqnCh[x1][0] < M[c_in][0]));
+  assert {:msg "12.1: The actions of actor 'Adjudicator' might not have mutually exclusive guards (#2)"} !((1 <= (C[x2] - R[x2])) && (1 <= (C[c_in] - R[c_in])) && (1 <= (C[x1] - R[x1])) && (1 <= (C[c_in] - R[c_in])) && (SqnCh[x1][0] < M[c_in][0]));
+}
+const unique Net#spl: Actor;
+const unique Net#pri: Actor;
+const unique Net#sec: Actor;
+const unique Net#adj: Actor;
+const unique Net#a: Chan (int);
+const unique Net#b: Chan (int);
+const unique Net#c: Chan (int);
+const unique Net#d: Chan (int);
+const unique Net#e: Chan (int);
+const unique Net#f: Chan (int);
+const unique Net#g: Chan (int);
+procedure Net#init#7()
+  modifies C, R, M, I, St, SqnCh, SqnAct;
+{
+  assume 0 <= I[Net#a];
+  assume I[Net#a] <= R[Net#a];
+  assume R[Net#a] <= C[Net#a];
+  assume 0 <= I[Net#b];
+  assume I[Net#b] <= R[Net#b];
+  assume R[Net#b] <= C[Net#b];
+  assume 0 <= I[Net#c];
+  assume I[Net#c] <= R[Net#c];
+  assume R[Net#c] <= C[Net#c];
+  assume 0 <= I[Net#d];
+  assume I[Net#d] <= R[Net#d];
+  assume R[Net#d] <= C[Net#d];
+  assume 0 <= I[Net#e];
+  assume I[Net#e] <= R[Net#e];
+  assume R[Net#e] <= C[Net#e];
+  assume 0 <= I[Net#f];
+  assume I[Net#f] <= R[Net#f];
+  assume R[Net#f] <= C[Net#f];
+  assume 0 <= I[Net#g];
+  assume I[Net#g] <= R[Net#g];
+  assume R[Net#g] <= C[Net#g];
+  assume I[Net#g] == R[Net#g];
   assume C[Net#a] == 0;
   assume R[Net#a] == 0;
   assume C[Net#b] == 0;
@@ -114,1213 +150,1264 @@ procedure Net#init#6()
   assume SqnAct[Net#pri] == 0;
   assume SqnAct[Net#sec] == 0;
   assume SqnAct[Net#adj] == 0;
-  M[Net#f][R[Net#f] + C[Net#f]] := 0;
+  M[Net#f][C[Net#f]] := 0;
   C[Net#f] := C[Net#f] + 1;
-  assert {:msg "  Network initialization might not establish the channel invariant"} R[Net#a] == (R[Net#b] + C[Net#b]);
-  assert {:msg "  Network initialization might not establish the channel invariant"} R[Net#a] == (R[Net#c] + C[Net#c]);
-  assert {:msg "  Network initialization might not establish the channel invariant"} R[Net#b] == (R[Net#d] + C[Net#d]);
-  assert {:msg "  Network initialization might not establish the channel invariant"} R[Net#c] == (R[Net#e] + C[Net#e]);
-  assert {:msg "  Network initialization might not establish the channel invariant"} (forall idx$: int :: 
-    (0 <= idx$) && (idx$ < (R[Net#b] + C[Net#b])) ==> (M[Net#b][idx$] == M[Net#a][idx$])
+  assert {:msg "41.15: Network initialization might not establish the channel invariant (#3)"} SqnAct[Net#spl] == R[Net#a];
+  assert {:msg "42.15: Network initialization might not establish the channel invariant (#4)"} SqnAct[Net#pri] == R[Net#b];
+  assert {:msg "43.15: Network initialization might not establish the channel invariant (#5)"} SqnAct[Net#sec] == R[Net#c];
+  assert {:msg "44.15: Network initialization might not establish the channel invariant (#6)"} SqnAct[Net#adj] == R[Net#e];
+  assert {:msg "46.16: Network initialization might not establish the channel invariant (#7)"} (forall i: int :: 
+    (0 <= i) && (i < C[Net#a]) ==> (SqnCh[Net#a][i] == i)
   );
-  assert {:msg "  Network initialization might not establish the channel invariant"} (forall idx$: int :: 
-    (0 <= idx$) && (idx$ < (R[Net#c] + C[Net#c])) ==> (M[Net#c][idx$] == M[Net#a][idx$])
+  assert {:msg "47.16: Network initialization might not establish the channel invariant (#8)"} (forall i: int :: 
+    (0 <= i) && (i < C[Net#b]) ==> (SqnCh[Net#b][i] == i)
   );
-  assert {:msg "  Network initialization might not establish the channel invariant"} (forall idx$: int :: 
-    (0 <= idx$) && (idx$ < (R[Net#d] + C[Net#d])) ==> (M[Net#d][idx$] == M[Net#b][idx$])
+  assert {:msg "48.16: Network initialization might not establish the channel invariant (#9)"} (forall i: int :: 
+    (0 <= i) && (i < C[Net#c]) ==> (SqnCh[Net#c][i] == i)
   );
-  assert {:msg "  Network initialization might not establish the channel invariant"} (forall idx$: int :: 
-    (0 <= idx$) && (idx$ < (R[Net#e] + C[Net#e])) ==> (M[Net#e][idx$] == M[Net#c][idx$])
+  assert {:msg "49.16: Network initialization might not establish the channel invariant (#10)"} (forall i: int :: 
+    (0 <= i) && (i < C[Net#d]) ==> (SqnCh[Net#d][i] == i)
   );
-  assert {:msg "  Network initialization might not establish the channel invariant"} (forall idx$: int :: 
-    (0 <= idx$) && (idx$ < (R[Net#a] + C[Net#a])) ==> (SqnCh[Net#a][idx$] == idx$)
+  assert {:msg "50.16: Network initialization might not establish the channel invariant (#11)"} (forall i: int :: 
+    (0 <= i) && (i < C[Net#e]) ==> (SqnCh[Net#e][i] == i)
   );
-  assert {:msg "  40.15: Network initialization might not establish the channel invariant"} SqnAct[Net#spl] == R[Net#a];
-  assert {:msg "  41.15: Network initialization might not establish the channel invariant"} SqnAct[Net#pri] == R[Net#b];
-  assert {:msg "  42.15: Network initialization might not establish the channel invariant"} SqnAct[Net#sec] == R[Net#c];
-  assert {:msg "  43.15: Network initialization might not establish the channel invariant"} SqnAct[Net#adj] == R[Net#e];
-  assert {:msg "  45.16: Network initialization might not establish the channel invariant"} (forall i: int :: 
-    (0 <= i) && (i < (R[Net#a] + C[Net#a])) ==> (SqnCh[Net#a][i] == i)
+  assert {:msg "51.16: Network initialization might not establish the channel invariant (#12)"} (forall i: int :: 
+    (0 <= i) && (i < C[Net#g]) ==> (SqnCh[Net#g][i] == i)
   );
-  assert {:msg "  46.16: Network initialization might not establish the channel invariant"} (forall i: int :: 
-    (0 <= i) && (i < (R[Net#b] + C[Net#b])) ==> (SqnCh[Net#b][i] == i)
+  assert {:msg "53.15: Network initialization might not establish the channel invariant (#13)"} (C[Net#f] - R[Net#f]) == 1;
+  assert {:msg "54.15: Network initialization might not establish the channel invariant (#14)"} C[Net#g] == R[Net#e];
+  assert {:msg "55.15: Network initialization might not establish the channel invariant (#15)"} R[Net#e] == M[Net#f][R[Net#f]];
+  assert {:msg "56.16: Network initialization might not establish the channel invariant (#16)"} (forall i: int :: 
+    (0 <= i) && (i < C[Net#g]) ==> (SqnCh[Net#g][i] == i)
   );
-  assert {:msg "  47.16: Network initialization might not establish the channel invariant"} (forall i: int :: 
-    (0 <= i) && (i < (R[Net#c] + C[Net#c])) ==> (SqnCh[Net#c][i] == i)
-  );
-  assert {:msg "  48.16: Network initialization might not establish the channel invariant"} (forall i: int :: 
-    (0 <= i) && (i < (R[Net#d] + C[Net#d])) ==> (SqnCh[Net#d][i] == i)
-  );
-  assert {:msg "  49.16: Network initialization might not establish the channel invariant"} (forall i: int :: 
-    (0 <= i) && (i < (R[Net#e] + C[Net#e])) ==> (SqnCh[Net#e][i] == i)
-  );
-  assert {:msg "  50.16: Network initialization might not establish the channel invariant"} (forall i: int :: 
-    (0 <= i) && (i < (R[Net#g] + C[Net#g])) ==> (SqnCh[Net#g][i] == i)
-  );
-  assert {:msg "  52.15: Network initialization might not establish the channel invariant"} C[Net#f] == 1;
-  assert {:msg "  53.15: Network initialization might not establish the channel invariant"} (R[Net#g] + C[Net#g]) == R[Net#e];
-  assert {:msg "  54.15: Network initialization might not establish the channel invariant"} R[Net#e] == M[Net#f][R[Net#f]];
-  assert {:msg "  55.16: Network initialization might not establish the channel invariant"} (forall i: int :: 
-    (0 <= i) && (i < (R[Net#g] + C[Net#g])) ==> (SqnCh[Net#g][i] == i)
-  );
-  if ((0 < R[Net#d]) && (0 < R[Net#e])) {
-    assert {:msg "  57.42: Network initialization might not establish the channel invariant"} M[Net#d][R[Net#d] - 1] <= M[Net#e][R[Net#e] - 1];
-  }
-  assert {:msg "  58.16: Network initialization might not establish the channel invariant"} (forall i: int :: 
+  assert {:msg "59.16: Network initialization might not establish the channel invariant (#17)"} (forall i: int :: 
     (0 <= i) && (i < R[Net#e]) ==> (M[Net#g][i] == M[Net#e][i])
   );
+  assert {:msg "Network initialization might not establish the channel invariant (#18)"} R[Net#a] == C[Net#b];
+  assert {:msg "Network initialization might not establish the channel invariant (#19)"} R[Net#a] == C[Net#c];
+  assert {:msg "Network initialization might not establish the channel invariant (#20)"} R[Net#b] == C[Net#d];
+  assert {:msg "Network initialization might not establish the channel invariant (#21)"} R[Net#c] == C[Net#e];
+  assert {:msg "Network initialization might not establish the channel invariant (#22)"} (forall idx$: int :: 
+    (0 <= idx$) && (idx$ < C[Net#b]) ==> (M[Net#b][idx$] == M[Net#a][idx$])
+  );
+  assert {:msg "Network initialization might not establish the channel invariant (#23)"} (forall idx$: int :: 
+    (0 <= idx$) && (idx$ < C[Net#c]) ==> (M[Net#c][idx$] == M[Net#a][idx$])
+  );
+  assert {:msg "Network initialization might not establish the channel invariant (#24)"} (forall idx$: int :: 
+    (0 <= idx$) && (idx$ < C[Net#d]) ==> (M[Net#d][idx$] == M[Net#b][idx$])
+  );
+  assert {:msg "Network initialization might not establish the channel invariant (#25)"} (forall idx$: int :: 
+    (0 <= idx$) && (idx$ < C[Net#e]) ==> (M[Net#e][idx$] == M[Net#c][idx$])
+  );
+  assert {:msg "Network initialization might not establish the channel invariant (#26)"} (forall idx$: int :: 
+    (0 <= idx$) && (idx$ < C[Net#a]) ==> (SqnCh[Net#a][idx$] == idx$)
+  );
+  I := R;
   C[Net#f] := C[Net#f] - 1;
-  assert {:msg "  38.13: Network initialization might not establish the network invariant"} R[Net#e] == M[Net#f][R[Net#f]];
+  assert {:msg "39.13: Network initialization might not establish the network invariant"} R[Net#e] == M[Net#f][R[Net#f]];
 }
-const unique Net#spl: Actor;
-const unique Net#pri: Actor;
-const unique Net#sec: Actor;
-const unique Net#adj: Actor;
-const unique Net#a: Chan (int);
-const unique Net#b: Chan (int);
-const unique Net#c: Chan (int);
-const unique Net#d: Chan (int);
-const unique Net#e: Chan (int);
-const unique Net#f: Chan (int);
-const unique Net#g: Chan (int);
-procedure Net#anon$3#entry#7()
-  modifies C, R, M, St, SqnCh, SqnAct;
-{
-  assume L[Net#a] == (1 * Base#L);
-  assume C[Net#a] == 0;
-  assume C[Net#b] == 0;
-  assume C[Net#c] == 0;
-  assume C[Net#d] == 0;
-  assume C[Net#e] == 0;
-  assume C[Net#f] == 0;
-  assume C[Net#g] == 0;
-  C[Net#f] := C[Net#f] + 1;
-  assume R[Net#e] == M[Net#f][R[Net#f]];
-  assume 0 <= R[Net#a];
-  assume 0 <= C[Net#a];
-  assume (R[Net#a] + C[Net#a]) <= L[Net#a];
-  assume 0 <= R[Net#b];
-  assume 0 <= C[Net#b];
-  assume 0 <= R[Net#c];
-  assume 0 <= C[Net#c];
-  assume 0 <= R[Net#d];
-  assume 0 <= C[Net#d];
-  assume 0 <= R[Net#e];
-  assume 0 <= C[Net#e];
-  assume 0 <= R[Net#f];
-  assume 0 <= C[Net#f];
-  assume 0 <= R[Net#g];
-  assume 0 <= C[Net#g];
-  assume R[Net#g] == 0;
-  assume R[Net#a] == (R[Net#b] + C[Net#b]);
-  assume R[Net#a] == (R[Net#c] + C[Net#c]);
-  assume R[Net#b] == (R[Net#d] + C[Net#d]);
-  assume R[Net#c] == (R[Net#e] + C[Net#e]);
-  assume (forall idx$: int :: 
-    (0 <= idx$) && (idx$ < (R[Net#b] + C[Net#b])) ==> (M[Net#b][idx$] == M[Net#a][idx$])
-  );
-  assume (forall idx$: int :: 
-    (0 <= idx$) && (idx$ < (R[Net#c] + C[Net#c])) ==> (M[Net#c][idx$] == M[Net#a][idx$])
-  );
-  assume (forall idx$: int :: 
-    (0 <= idx$) && (idx$ < (R[Net#d] + C[Net#d])) ==> (M[Net#d][idx$] == M[Net#b][idx$])
-  );
-  assume (forall idx$: int :: 
-    (0 <= idx$) && (idx$ < (R[Net#e] + C[Net#e])) ==> (M[Net#e][idx$] == M[Net#c][idx$])
-  );
-  assume (forall idx$: int :: 
-    (0 <= idx$) && (idx$ < (R[Net#a] + C[Net#a])) ==> (SqnCh[Net#a][idx$] == idx$)
-  );
-  assume SqnAct[Net#spl] == R[Net#a];
-  assume SqnAct[Net#pri] == R[Net#b];
-  assume SqnAct[Net#sec] == R[Net#c];
-  assume SqnAct[Net#adj] == R[Net#e];
-  assume (forall i: int :: 
-    (0 <= i) && (i < (R[Net#a] + C[Net#a])) ==> (SqnCh[Net#a][i] == i)
-  );
-  assume (forall i: int :: 
-    (0 <= i) && (i < (R[Net#b] + C[Net#b])) ==> (SqnCh[Net#b][i] == i)
-  );
-  assume (forall i: int :: 
-    (0 <= i) && (i < (R[Net#c] + C[Net#c])) ==> (SqnCh[Net#c][i] == i)
-  );
-  assume (forall i: int :: 
-    (0 <= i) && (i < (R[Net#d] + C[Net#d])) ==> (SqnCh[Net#d][i] == i)
-  );
-  assume (forall i: int :: 
-    (0 <= i) && (i < (R[Net#e] + C[Net#e])) ==> (SqnCh[Net#e][i] == i)
-  );
-  assume (forall i: int :: 
-    (0 <= i) && (i < (R[Net#g] + C[Net#g])) ==> (SqnCh[Net#g][i] == i)
-  );
-  assume C[Net#f] == 1;
-  assume (R[Net#g] + C[Net#g]) == R[Net#e];
-  assume R[Net#e] == M[Net#f][R[Net#f]];
-  assume (forall i: int :: 
-    (0 <= i) && (i < (R[Net#g] + C[Net#g])) ==> (SqnCh[Net#g][i] == i)
-  );
-  if ((0 < R[Net#d]) && (0 < R[Net#e])) {
-    assume M[Net#d][R[Net#d] - 1] <= M[Net#e][R[Net#e] - 1];
-  }
-  assume (forall i: int :: 
-    (0 <= i) && (i < R[Net#e]) ==> (M[Net#g][i] == M[Net#e][i])
-  );
-  assert {:msg "  Channel invariant might not hold on action entry (#0)"} R[Net#a] == (R[Net#b] + C[Net#b]);
-  assert {:msg "  Channel invariant might not hold on action entry (#1)"} R[Net#a] == (R[Net#c] + C[Net#c]);
-  assert {:msg "  Channel invariant might not hold on action entry (#2)"} R[Net#b] == (R[Net#d] + C[Net#d]);
-  assert {:msg "  Channel invariant might not hold on action entry (#3)"} R[Net#c] == (R[Net#e] + C[Net#e]);
-  assert {:msg "  Channel invariant might not hold on action entry (#4)"} (forall idx$: int :: 
-    (0 <= idx$) && (idx$ < (R[Net#b] + C[Net#b])) ==> (M[Net#b][idx$] == M[Net#a][idx$])
-  );
-  assert {:msg "  Channel invariant might not hold on action entry (#5)"} (forall idx$: int :: 
-    (0 <= idx$) && (idx$ < (R[Net#c] + C[Net#c])) ==> (M[Net#c][idx$] == M[Net#a][idx$])
-  );
-  assert {:msg "  Channel invariant might not hold on action entry (#6)"} (forall idx$: int :: 
-    (0 <= idx$) && (idx$ < (R[Net#d] + C[Net#d])) ==> (M[Net#d][idx$] == M[Net#b][idx$])
-  );
-  assert {:msg "  Channel invariant might not hold on action entry (#7)"} (forall idx$: int :: 
-    (0 <= idx$) && (idx$ < (R[Net#e] + C[Net#e])) ==> (M[Net#e][idx$] == M[Net#c][idx$])
-  );
-  assert {:msg "  Channel invariant might not hold on action entry (#8)"} (forall idx$: int :: 
-    (0 <= idx$) && (idx$ < (R[Net#a] + C[Net#a])) ==> (SqnCh[Net#a][idx$] == idx$)
-  );
-  assert {:msg "  40.15: Channel invariant might not hold on action entry (#9)"} SqnAct[Net#spl] == R[Net#a];
-  assert {:msg "  41.15: Channel invariant might not hold on action entry (#10)"} SqnAct[Net#pri] == R[Net#b];
-  assert {:msg "  42.15: Channel invariant might not hold on action entry (#11)"} SqnAct[Net#sec] == R[Net#c];
-  assert {:msg "  43.15: Channel invariant might not hold on action entry (#12)"} SqnAct[Net#adj] == R[Net#e];
-  assert {:msg "  45.16: Channel invariant might not hold on action entry (#13)"} (forall i: int :: 
-    (0 <= i) && (i < (R[Net#a] + C[Net#a])) ==> (SqnCh[Net#a][i] == i)
-  );
-  assert {:msg "  46.16: Channel invariant might not hold on action entry (#14)"} (forall i: int :: 
-    (0 <= i) && (i < (R[Net#b] + C[Net#b])) ==> (SqnCh[Net#b][i] == i)
-  );
-  assert {:msg "  47.16: Channel invariant might not hold on action entry (#15)"} (forall i: int :: 
-    (0 <= i) && (i < (R[Net#c] + C[Net#c])) ==> (SqnCh[Net#c][i] == i)
-  );
-  assert {:msg "  48.16: Channel invariant might not hold on action entry (#16)"} (forall i: int :: 
-    (0 <= i) && (i < (R[Net#d] + C[Net#d])) ==> (SqnCh[Net#d][i] == i)
-  );
-  assert {:msg "  49.16: Channel invariant might not hold on action entry (#17)"} (forall i: int :: 
-    (0 <= i) && (i < (R[Net#e] + C[Net#e])) ==> (SqnCh[Net#e][i] == i)
-  );
-  assert {:msg "  50.16: Channel invariant might not hold on action entry (#18)"} (forall i: int :: 
-    (0 <= i) && (i < (R[Net#g] + C[Net#g])) ==> (SqnCh[Net#g][i] == i)
-  );
-  assert {:msg "  52.15: Channel invariant might not hold on action entry (#19)"} C[Net#f] == 1;
-  assert {:msg "  53.15: Channel invariant might not hold on action entry (#20)"} (R[Net#g] + C[Net#g]) == R[Net#e];
-  assert {:msg "  54.15: Channel invariant might not hold on action entry (#21)"} R[Net#e] == M[Net#f][R[Net#f]];
-  assert {:msg "  55.16: Channel invariant might not hold on action entry (#22)"} (forall i: int :: 
-    (0 <= i) && (i < (R[Net#g] + C[Net#g])) ==> (SqnCh[Net#g][i] == i)
-  );
-  if ((0 < R[Net#d]) && (0 < R[Net#e])) {
-    assert {:msg "  57.42: Channel invariant might not hold on action entry (#23)"} M[Net#d][R[Net#d] - 1] <= M[Net#e][R[Net#e] - 1];
-  }
-  assert {:msg "  58.16: Channel invariant might not hold on action entry (#24)"} (forall i: int :: 
-    (0 <= i) && (i < R[Net#e]) ==> (M[Net#g][i] == M[Net#e][i])
-  );
-}
-procedure Net#anon$3#Split#anon$1#8()
-  modifies C, R, M, St, SqnCh, SqnAct;
+procedure Net##Split#anon$1#8()
+  modifies C, R, M, I, St, SqnCh, SqnAct;
 {
   var St#next: State;
   var in#i: int;
-  assume L[Net#a] == (1 * Base#L);
-  assume 0 <= R[Net#a];
-  assume 0 <= C[Net#a];
-  assume (R[Net#a] + C[Net#a]) <= L[Net#a];
-  assume 0 <= R[Net#b];
-  assume 0 <= C[Net#b];
-  assume 0 <= R[Net#c];
-  assume 0 <= C[Net#c];
-  assume 0 <= R[Net#d];
-  assume 0 <= C[Net#d];
-  assume 0 <= R[Net#e];
-  assume 0 <= C[Net#e];
-  assume 0 <= R[Net#f];
-  assume 0 <= C[Net#f];
-  assume 0 <= R[Net#g];
-  assume 0 <= C[Net#g];
-  assume R[Net#g] == 0;
-  assume R[Net#a] == (R[Net#b] + C[Net#b]);
-  assume R[Net#a] == (R[Net#c] + C[Net#c]);
-  assume R[Net#b] == (R[Net#d] + C[Net#d]);
-  assume R[Net#c] == (R[Net#e] + C[Net#e]);
-  assume (forall idx$: int :: 
-    (0 <= idx$) && (idx$ < (R[Net#b] + C[Net#b])) ==> (M[Net#b][idx$] == M[Net#a][idx$])
-  );
-  assume (forall idx$: int :: 
-    (0 <= idx$) && (idx$ < (R[Net#c] + C[Net#c])) ==> (M[Net#c][idx$] == M[Net#a][idx$])
-  );
-  assume (forall idx$: int :: 
-    (0 <= idx$) && (idx$ < (R[Net#d] + C[Net#d])) ==> (M[Net#d][idx$] == M[Net#b][idx$])
-  );
-  assume (forall idx$: int :: 
-    (0 <= idx$) && (idx$ < (R[Net#e] + C[Net#e])) ==> (M[Net#e][idx$] == M[Net#c][idx$])
-  );
-  assume (forall idx$: int :: 
-    (0 <= idx$) && (idx$ < (R[Net#a] + C[Net#a])) ==> (SqnCh[Net#a][idx$] == idx$)
-  );
+  assume 0 <= I[Net#a];
+  assume I[Net#a] <= R[Net#a];
+  assume R[Net#a] <= C[Net#a];
+  assume 0 <= I[Net#b];
+  assume I[Net#b] <= R[Net#b];
+  assume R[Net#b] <= C[Net#b];
+  assume 0 <= I[Net#c];
+  assume I[Net#c] <= R[Net#c];
+  assume R[Net#c] <= C[Net#c];
+  assume 0 <= I[Net#d];
+  assume I[Net#d] <= R[Net#d];
+  assume R[Net#d] <= C[Net#d];
+  assume 0 <= I[Net#e];
+  assume I[Net#e] <= R[Net#e];
+  assume R[Net#e] <= C[Net#e];
+  assume 0 <= I[Net#f];
+  assume I[Net#f] <= R[Net#f];
+  assume R[Net#f] <= C[Net#f];
+  assume 0 <= I[Net#g];
+  assume I[Net#g] <= R[Net#g];
+  assume R[Net#g] <= C[Net#g];
+  assume I[Net#g] == R[Net#g];
   assume SqnAct[Net#spl] == R[Net#a];
   assume SqnAct[Net#pri] == R[Net#b];
   assume SqnAct[Net#sec] == R[Net#c];
   assume SqnAct[Net#adj] == R[Net#e];
   assume (forall i: int :: 
-    (0 <= i) && (i < (R[Net#a] + C[Net#a])) ==> (SqnCh[Net#a][i] == i)
+    (0 <= i) && (i < C[Net#a]) ==> (SqnCh[Net#a][i] == i)
   );
   assume (forall i: int :: 
-    (0 <= i) && (i < (R[Net#b] + C[Net#b])) ==> (SqnCh[Net#b][i] == i)
+    (0 <= i) && (i < C[Net#b]) ==> (SqnCh[Net#b][i] == i)
   );
   assume (forall i: int :: 
-    (0 <= i) && (i < (R[Net#c] + C[Net#c])) ==> (SqnCh[Net#c][i] == i)
+    (0 <= i) && (i < C[Net#c]) ==> (SqnCh[Net#c][i] == i)
   );
   assume (forall i: int :: 
-    (0 <= i) && (i < (R[Net#d] + C[Net#d])) ==> (SqnCh[Net#d][i] == i)
+    (0 <= i) && (i < C[Net#d]) ==> (SqnCh[Net#d][i] == i)
   );
   assume (forall i: int :: 
-    (0 <= i) && (i < (R[Net#e] + C[Net#e])) ==> (SqnCh[Net#e][i] == i)
+    (0 <= i) && (i < C[Net#e]) ==> (SqnCh[Net#e][i] == i)
   );
   assume (forall i: int :: 
-    (0 <= i) && (i < (R[Net#g] + C[Net#g])) ==> (SqnCh[Net#g][i] == i)
+    (0 <= i) && (i < C[Net#g]) ==> (SqnCh[Net#g][i] == i)
   );
-  assume C[Net#f] == 1;
-  assume (R[Net#g] + C[Net#g]) == R[Net#e];
+  assume (C[Net#f] - R[Net#f]) == 1;
+  assume C[Net#g] == R[Net#e];
   assume R[Net#e] == M[Net#f][R[Net#f]];
   assume (forall i: int :: 
-    (0 <= i) && (i < (R[Net#g] + C[Net#g])) ==> (SqnCh[Net#g][i] == i)
+    (0 <= i) && (i < C[Net#g]) ==> (SqnCh[Net#g][i] == i)
   );
-  if ((0 < R[Net#d]) && (0 < R[Net#e])) {
-    assume M[Net#d][R[Net#d] - 1] <= M[Net#e][R[Net#e] - 1];
-  }
   assume (forall i: int :: 
     (0 <= i) && (i < R[Net#e]) ==> (M[Net#g][i] == M[Net#e][i])
   );
+  assume R[Net#a] == C[Net#b];
+  assume R[Net#a] == C[Net#c];
+  assume R[Net#b] == C[Net#d];
+  assume R[Net#c] == C[Net#e];
+  assume (forall idx$: int :: 
+    (0 <= idx$) && (idx$ < C[Net#b]) ==> (M[Net#b][idx$] == M[Net#a][idx$])
+  );
+  assume (forall idx$: int :: 
+    (0 <= idx$) && (idx$ < C[Net#c]) ==> (M[Net#c][idx$] == M[Net#a][idx$])
+  );
+  assume (forall idx$: int :: 
+    (0 <= idx$) && (idx$ < C[Net#d]) ==> (M[Net#d][idx$] == M[Net#b][idx$])
+  );
+  assume (forall idx$: int :: 
+    (0 <= idx$) && (idx$ < C[Net#e]) ==> (M[Net#e][idx$] == M[Net#c][idx$])
+  );
+  assume (forall idx$: int :: 
+    (0 <= idx$) && (idx$ < C[Net#a]) ==> (SqnCh[Net#a][idx$] == idx$)
+  );
   assume true;
-  assume 1 <= C[Net#a];
+  assume 1 <= (C[Net#a] - R[Net#a]);
   in#i := M[Net#a][R[Net#a]];
   R[Net#a] := R[Net#a] + 1;
-  C[Net#a] := C[Net#a] - 1;
-  M[Net#b][R[Net#b] + C[Net#b]] := in#i;
-  SqnCh[Net#b][R[Net#b] + C[Net#b]] := SqnAct[Net#spl];
+  M[Net#b][C[Net#b]] := in#i;
+  SqnCh[Net#b][C[Net#b]] := SqnAct[Net#spl];
   C[Net#b] := C[Net#b] + 1;
-  M[Net#c][R[Net#c] + C[Net#c]] := in#i;
-  SqnCh[Net#c][R[Net#c] + C[Net#c]] := SqnAct[Net#spl];
+  M[Net#c][C[Net#c]] := in#i;
+  SqnCh[Net#c][C[Net#c]] := SqnAct[Net#spl];
   C[Net#c] := C[Net#c] + 1;
   SqnAct[Net#spl] := SqnAct[Net#spl] + 1;
-  assert {:msg "  Action at 8.3 ('anon$1') for actor instance 'spl' might not preserve the channel invariant (#25)"} R[Net#a] == (R[Net#b] + C[Net#b]);
-  assert {:msg "  Action at 8.3 ('anon$1') for actor instance 'spl' might not preserve the channel invariant (#26)"} R[Net#a] == (R[Net#c] + C[Net#c]);
-  assert {:msg "  Action at 8.3 ('anon$1') for actor instance 'spl' might not preserve the channel invariant (#27)"} R[Net#b] == (R[Net#d] + C[Net#d]);
-  assert {:msg "  Action at 8.3 ('anon$1') for actor instance 'spl' might not preserve the channel invariant (#28)"} R[Net#c] == (R[Net#e] + C[Net#e]);
-  assert {:msg "  Action at 8.3 ('anon$1') for actor instance 'spl' might not preserve the channel invariant (#29)"} (forall idx$: int :: 
-    (0 <= idx$) && (idx$ < (R[Net#b] + C[Net#b])) ==> (M[Net#b][idx$] == M[Net#a][idx$])
+  assert {:msg "41.15: Action at 8.3 ('anon$1') for actor instance 'spl' might not preserve the channel invariant (#27)"} SqnAct[Net#spl] == R[Net#a];
+  assert {:msg "42.15: Action at 8.3 ('anon$1') for actor instance 'spl' might not preserve the channel invariant (#28)"} SqnAct[Net#pri] == R[Net#b];
+  assert {:msg "43.15: Action at 8.3 ('anon$1') for actor instance 'spl' might not preserve the channel invariant (#29)"} SqnAct[Net#sec] == R[Net#c];
+  assert {:msg "44.15: Action at 8.3 ('anon$1') for actor instance 'spl' might not preserve the channel invariant (#30)"} SqnAct[Net#adj] == R[Net#e];
+  assert {:msg "46.16: Action at 8.3 ('anon$1') for actor instance 'spl' might not preserve the channel invariant (#31)"} (forall i: int :: 
+    (0 <= i) && (i < C[Net#a]) ==> (SqnCh[Net#a][i] == i)
   );
-  assert {:msg "  Action at 8.3 ('anon$1') for actor instance 'spl' might not preserve the channel invariant (#30)"} (forall idx$: int :: 
-    (0 <= idx$) && (idx$ < (R[Net#c] + C[Net#c])) ==> (M[Net#c][idx$] == M[Net#a][idx$])
+  assert {:msg "47.16: Action at 8.3 ('anon$1') for actor instance 'spl' might not preserve the channel invariant (#32)"} (forall i: int :: 
+    (0 <= i) && (i < C[Net#b]) ==> (SqnCh[Net#b][i] == i)
   );
-  assert {:msg "  Action at 8.3 ('anon$1') for actor instance 'spl' might not preserve the channel invariant (#31)"} (forall idx$: int :: 
-    (0 <= idx$) && (idx$ < (R[Net#d] + C[Net#d])) ==> (M[Net#d][idx$] == M[Net#b][idx$])
+  assert {:msg "48.16: Action at 8.3 ('anon$1') for actor instance 'spl' might not preserve the channel invariant (#33)"} (forall i: int :: 
+    (0 <= i) && (i < C[Net#c]) ==> (SqnCh[Net#c][i] == i)
   );
-  assert {:msg "  Action at 8.3 ('anon$1') for actor instance 'spl' might not preserve the channel invariant (#32)"} (forall idx$: int :: 
-    (0 <= idx$) && (idx$ < (R[Net#e] + C[Net#e])) ==> (M[Net#e][idx$] == M[Net#c][idx$])
+  assert {:msg "49.16: Action at 8.3 ('anon$1') for actor instance 'spl' might not preserve the channel invariant (#34)"} (forall i: int :: 
+    (0 <= i) && (i < C[Net#d]) ==> (SqnCh[Net#d][i] == i)
   );
-  assert {:msg "  Action at 8.3 ('anon$1') for actor instance 'spl' might not preserve the channel invariant (#33)"} (forall idx$: int :: 
-    (0 <= idx$) && (idx$ < (R[Net#a] + C[Net#a])) ==> (SqnCh[Net#a][idx$] == idx$)
+  assert {:msg "50.16: Action at 8.3 ('anon$1') for actor instance 'spl' might not preserve the channel invariant (#35)"} (forall i: int :: 
+    (0 <= i) && (i < C[Net#e]) ==> (SqnCh[Net#e][i] == i)
   );
-  assert {:msg "  40.15: Action at 8.3 ('anon$1') for actor instance 'spl' might not preserve the channel invariant (#34)"} SqnAct[Net#spl] == R[Net#a];
-  assert {:msg "  41.15: Action at 8.3 ('anon$1') for actor instance 'spl' might not preserve the channel invariant (#35)"} SqnAct[Net#pri] == R[Net#b];
-  assert {:msg "  42.15: Action at 8.3 ('anon$1') for actor instance 'spl' might not preserve the channel invariant (#36)"} SqnAct[Net#sec] == R[Net#c];
-  assert {:msg "  43.15: Action at 8.3 ('anon$1') for actor instance 'spl' might not preserve the channel invariant (#37)"} SqnAct[Net#adj] == R[Net#e];
-  assert {:msg "  45.16: Action at 8.3 ('anon$1') for actor instance 'spl' might not preserve the channel invariant (#38)"} (forall i: int :: 
-    (0 <= i) && (i < (R[Net#a] + C[Net#a])) ==> (SqnCh[Net#a][i] == i)
+  assert {:msg "51.16: Action at 8.3 ('anon$1') for actor instance 'spl' might not preserve the channel invariant (#36)"} (forall i: int :: 
+    (0 <= i) && (i < C[Net#g]) ==> (SqnCh[Net#g][i] == i)
   );
-  assert {:msg "  46.16: Action at 8.3 ('anon$1') for actor instance 'spl' might not preserve the channel invariant (#39)"} (forall i: int :: 
-    (0 <= i) && (i < (R[Net#b] + C[Net#b])) ==> (SqnCh[Net#b][i] == i)
+  assert {:msg "53.15: Action at 8.3 ('anon$1') for actor instance 'spl' might not preserve the channel invariant (#37)"} (C[Net#f] - R[Net#f]) == 1;
+  assert {:msg "54.15: Action at 8.3 ('anon$1') for actor instance 'spl' might not preserve the channel invariant (#38)"} C[Net#g] == R[Net#e];
+  assert {:msg "55.15: Action at 8.3 ('anon$1') for actor instance 'spl' might not preserve the channel invariant (#39)"} R[Net#e] == M[Net#f][R[Net#f]];
+  assert {:msg "56.16: Action at 8.3 ('anon$1') for actor instance 'spl' might not preserve the channel invariant (#40)"} (forall i: int :: 
+    (0 <= i) && (i < C[Net#g]) ==> (SqnCh[Net#g][i] == i)
   );
-  assert {:msg "  47.16: Action at 8.3 ('anon$1') for actor instance 'spl' might not preserve the channel invariant (#40)"} (forall i: int :: 
-    (0 <= i) && (i < (R[Net#c] + C[Net#c])) ==> (SqnCh[Net#c][i] == i)
-  );
-  assert {:msg "  48.16: Action at 8.3 ('anon$1') for actor instance 'spl' might not preserve the channel invariant (#41)"} (forall i: int :: 
-    (0 <= i) && (i < (R[Net#d] + C[Net#d])) ==> (SqnCh[Net#d][i] == i)
-  );
-  assert {:msg "  49.16: Action at 8.3 ('anon$1') for actor instance 'spl' might not preserve the channel invariant (#42)"} (forall i: int :: 
-    (0 <= i) && (i < (R[Net#e] + C[Net#e])) ==> (SqnCh[Net#e][i] == i)
-  );
-  assert {:msg "  50.16: Action at 8.3 ('anon$1') for actor instance 'spl' might not preserve the channel invariant (#43)"} (forall i: int :: 
-    (0 <= i) && (i < (R[Net#g] + C[Net#g])) ==> (SqnCh[Net#g][i] == i)
-  );
-  assert {:msg "  52.15: Action at 8.3 ('anon$1') for actor instance 'spl' might not preserve the channel invariant (#44)"} C[Net#f] == 1;
-  assert {:msg "  53.15: Action at 8.3 ('anon$1') for actor instance 'spl' might not preserve the channel invariant (#45)"} (R[Net#g] + C[Net#g]) == R[Net#e];
-  assert {:msg "  54.15: Action at 8.3 ('anon$1') for actor instance 'spl' might not preserve the channel invariant (#46)"} R[Net#e] == M[Net#f][R[Net#f]];
-  assert {:msg "  55.16: Action at 8.3 ('anon$1') for actor instance 'spl' might not preserve the channel invariant (#47)"} (forall i: int :: 
-    (0 <= i) && (i < (R[Net#g] + C[Net#g])) ==> (SqnCh[Net#g][i] == i)
-  );
-  if ((0 < R[Net#d]) && (0 < R[Net#e])) {
-    assert {:msg "  57.42: Action at 8.3 ('anon$1') for actor instance 'spl' might not preserve the channel invariant (#48)"} M[Net#d][R[Net#d] - 1] <= M[Net#e][R[Net#e] - 1];
-  }
-  assert {:msg "  58.16: Action at 8.3 ('anon$1') for actor instance 'spl' might not preserve the channel invariant (#49)"} (forall i: int :: 
+  assert {:msg "59.16: Action at 8.3 ('anon$1') for actor instance 'spl' might not preserve the channel invariant (#41)"} (forall i: int :: 
     (0 <= i) && (i < R[Net#e]) ==> (M[Net#g][i] == M[Net#e][i])
   );
+  assert {:msg "Action at 8.3 ('anon$1') for actor instance 'spl' might not preserve the channel invariant (#42)"} R[Net#a] == C[Net#b];
+  assert {:msg "Action at 8.3 ('anon$1') for actor instance 'spl' might not preserve the channel invariant (#43)"} R[Net#a] == C[Net#c];
+  assert {:msg "Action at 8.3 ('anon$1') for actor instance 'spl' might not preserve the channel invariant (#44)"} R[Net#b] == C[Net#d];
+  assert {:msg "Action at 8.3 ('anon$1') for actor instance 'spl' might not preserve the channel invariant (#45)"} R[Net#c] == C[Net#e];
+  assert {:msg "Action at 8.3 ('anon$1') for actor instance 'spl' might not preserve the channel invariant (#46)"} (forall idx$: int :: 
+    (0 <= idx$) && (idx$ < C[Net#b]) ==> (M[Net#b][idx$] == M[Net#a][idx$])
+  );
+  assert {:msg "Action at 8.3 ('anon$1') for actor instance 'spl' might not preserve the channel invariant (#47)"} (forall idx$: int :: 
+    (0 <= idx$) && (idx$ < C[Net#c]) ==> (M[Net#c][idx$] == M[Net#a][idx$])
+  );
+  assert {:msg "Action at 8.3 ('anon$1') for actor instance 'spl' might not preserve the channel invariant (#48)"} (forall idx$: int :: 
+    (0 <= idx$) && (idx$ < C[Net#d]) ==> (M[Net#d][idx$] == M[Net#b][idx$])
+  );
+  assert {:msg "Action at 8.3 ('anon$1') for actor instance 'spl' might not preserve the channel invariant (#49)"} (forall idx$: int :: 
+    (0 <= idx$) && (idx$ < C[Net#e]) ==> (M[Net#e][idx$] == M[Net#c][idx$])
+  );
+  assert {:msg "Action at 8.3 ('anon$1') for actor instance 'spl' might not preserve the channel invariant (#50)"} (forall idx$: int :: 
+    (0 <= idx$) && (idx$ < C[Net#a]) ==> (SqnCh[Net#a][idx$] == idx$)
+  );
 }
-procedure Net#anon$3#Rep#anon$0#9()
-  modifies C, R, M, St, SqnCh, SqnAct;
+procedure Net##Rep#anon$0#9()
+  modifies C, R, M, I, St, SqnCh, SqnAct;
 {
   var St#next: State;
   var in#i: int;
-  assume L[Net#a] == (1 * Base#L);
-  assume 0 <= R[Net#a];
-  assume 0 <= C[Net#a];
-  assume (R[Net#a] + C[Net#a]) <= L[Net#a];
-  assume 0 <= R[Net#b];
-  assume 0 <= C[Net#b];
-  assume 0 <= R[Net#c];
-  assume 0 <= C[Net#c];
-  assume 0 <= R[Net#d];
-  assume 0 <= C[Net#d];
-  assume 0 <= R[Net#e];
-  assume 0 <= C[Net#e];
-  assume 0 <= R[Net#f];
-  assume 0 <= C[Net#f];
-  assume 0 <= R[Net#g];
-  assume 0 <= C[Net#g];
-  assume R[Net#g] == 0;
-  assume R[Net#a] == (R[Net#b] + C[Net#b]);
-  assume R[Net#a] == (R[Net#c] + C[Net#c]);
-  assume R[Net#b] == (R[Net#d] + C[Net#d]);
-  assume R[Net#c] == (R[Net#e] + C[Net#e]);
-  assume (forall idx$: int :: 
-    (0 <= idx$) && (idx$ < (R[Net#b] + C[Net#b])) ==> (M[Net#b][idx$] == M[Net#a][idx$])
-  );
-  assume (forall idx$: int :: 
-    (0 <= idx$) && (idx$ < (R[Net#c] + C[Net#c])) ==> (M[Net#c][idx$] == M[Net#a][idx$])
-  );
-  assume (forall idx$: int :: 
-    (0 <= idx$) && (idx$ < (R[Net#d] + C[Net#d])) ==> (M[Net#d][idx$] == M[Net#b][idx$])
-  );
-  assume (forall idx$: int :: 
-    (0 <= idx$) && (idx$ < (R[Net#e] + C[Net#e])) ==> (M[Net#e][idx$] == M[Net#c][idx$])
-  );
-  assume (forall idx$: int :: 
-    (0 <= idx$) && (idx$ < (R[Net#a] + C[Net#a])) ==> (SqnCh[Net#a][idx$] == idx$)
-  );
+  assume 0 <= I[Net#a];
+  assume I[Net#a] <= R[Net#a];
+  assume R[Net#a] <= C[Net#a];
+  assume 0 <= I[Net#b];
+  assume I[Net#b] <= R[Net#b];
+  assume R[Net#b] <= C[Net#b];
+  assume 0 <= I[Net#c];
+  assume I[Net#c] <= R[Net#c];
+  assume R[Net#c] <= C[Net#c];
+  assume 0 <= I[Net#d];
+  assume I[Net#d] <= R[Net#d];
+  assume R[Net#d] <= C[Net#d];
+  assume 0 <= I[Net#e];
+  assume I[Net#e] <= R[Net#e];
+  assume R[Net#e] <= C[Net#e];
+  assume 0 <= I[Net#f];
+  assume I[Net#f] <= R[Net#f];
+  assume R[Net#f] <= C[Net#f];
+  assume 0 <= I[Net#g];
+  assume I[Net#g] <= R[Net#g];
+  assume R[Net#g] <= C[Net#g];
+  assume I[Net#g] == R[Net#g];
   assume SqnAct[Net#spl] == R[Net#a];
   assume SqnAct[Net#pri] == R[Net#b];
   assume SqnAct[Net#sec] == R[Net#c];
   assume SqnAct[Net#adj] == R[Net#e];
   assume (forall i: int :: 
-    (0 <= i) && (i < (R[Net#a] + C[Net#a])) ==> (SqnCh[Net#a][i] == i)
+    (0 <= i) && (i < C[Net#a]) ==> (SqnCh[Net#a][i] == i)
   );
   assume (forall i: int :: 
-    (0 <= i) && (i < (R[Net#b] + C[Net#b])) ==> (SqnCh[Net#b][i] == i)
+    (0 <= i) && (i < C[Net#b]) ==> (SqnCh[Net#b][i] == i)
   );
   assume (forall i: int :: 
-    (0 <= i) && (i < (R[Net#c] + C[Net#c])) ==> (SqnCh[Net#c][i] == i)
+    (0 <= i) && (i < C[Net#c]) ==> (SqnCh[Net#c][i] == i)
   );
   assume (forall i: int :: 
-    (0 <= i) && (i < (R[Net#d] + C[Net#d])) ==> (SqnCh[Net#d][i] == i)
+    (0 <= i) && (i < C[Net#d]) ==> (SqnCh[Net#d][i] == i)
   );
   assume (forall i: int :: 
-    (0 <= i) && (i < (R[Net#e] + C[Net#e])) ==> (SqnCh[Net#e][i] == i)
+    (0 <= i) && (i < C[Net#e]) ==> (SqnCh[Net#e][i] == i)
   );
   assume (forall i: int :: 
-    (0 <= i) && (i < (R[Net#g] + C[Net#g])) ==> (SqnCh[Net#g][i] == i)
+    (0 <= i) && (i < C[Net#g]) ==> (SqnCh[Net#g][i] == i)
   );
-  assume C[Net#f] == 1;
-  assume (R[Net#g] + C[Net#g]) == R[Net#e];
+  assume (C[Net#f] - R[Net#f]) == 1;
+  assume C[Net#g] == R[Net#e];
   assume R[Net#e] == M[Net#f][R[Net#f]];
   assume (forall i: int :: 
-    (0 <= i) && (i < (R[Net#g] + C[Net#g])) ==> (SqnCh[Net#g][i] == i)
+    (0 <= i) && (i < C[Net#g]) ==> (SqnCh[Net#g][i] == i)
   );
-  if ((0 < R[Net#d]) && (0 < R[Net#e])) {
-    assume M[Net#d][R[Net#d] - 1] <= M[Net#e][R[Net#e] - 1];
-  }
   assume (forall i: int :: 
     (0 <= i) && (i < R[Net#e]) ==> (M[Net#g][i] == M[Net#e][i])
   );
+  assume R[Net#a] == C[Net#b];
+  assume R[Net#a] == C[Net#c];
+  assume R[Net#b] == C[Net#d];
+  assume R[Net#c] == C[Net#e];
+  assume (forall idx$: int :: 
+    (0 <= idx$) && (idx$ < C[Net#b]) ==> (M[Net#b][idx$] == M[Net#a][idx$])
+  );
+  assume (forall idx$: int :: 
+    (0 <= idx$) && (idx$ < C[Net#c]) ==> (M[Net#c][idx$] == M[Net#a][idx$])
+  );
+  assume (forall idx$: int :: 
+    (0 <= idx$) && (idx$ < C[Net#d]) ==> (M[Net#d][idx$] == M[Net#b][idx$])
+  );
+  assume (forall idx$: int :: 
+    (0 <= idx$) && (idx$ < C[Net#e]) ==> (M[Net#e][idx$] == M[Net#c][idx$])
+  );
+  assume (forall idx$: int :: 
+    (0 <= idx$) && (idx$ < C[Net#a]) ==> (SqnCh[Net#a][idx$] == idx$)
+  );
   assume true;
-  assume 1 <= C[Net#b];
+  assume 1 <= (C[Net#b] - R[Net#b]);
   in#i := M[Net#b][R[Net#b]];
   R[Net#b] := R[Net#b] + 1;
-  C[Net#b] := C[Net#b] - 1;
-  M[Net#d][R[Net#d] + C[Net#d]] := in#i;
-  SqnCh[Net#d][R[Net#d] + C[Net#d]] := SqnAct[Net#pri];
+  M[Net#d][C[Net#d]] := in#i;
+  SqnCh[Net#d][C[Net#d]] := SqnAct[Net#pri];
   C[Net#d] := C[Net#d] + 1;
   SqnAct[Net#pri] := SqnAct[Net#pri] + 1;
-  assert {:msg "  Action at 3.3 ('anon$0') for actor instance 'pri' might not preserve the channel invariant (#50)"} R[Net#a] == (R[Net#b] + C[Net#b]);
-  assert {:msg "  Action at 3.3 ('anon$0') for actor instance 'pri' might not preserve the channel invariant (#51)"} R[Net#a] == (R[Net#c] + C[Net#c]);
-  assert {:msg "  Action at 3.3 ('anon$0') for actor instance 'pri' might not preserve the channel invariant (#52)"} R[Net#b] == (R[Net#d] + C[Net#d]);
-  assert {:msg "  Action at 3.3 ('anon$0') for actor instance 'pri' might not preserve the channel invariant (#53)"} R[Net#c] == (R[Net#e] + C[Net#e]);
-  assert {:msg "  Action at 3.3 ('anon$0') for actor instance 'pri' might not preserve the channel invariant (#54)"} (forall idx$: int :: 
-    (0 <= idx$) && (idx$ < (R[Net#b] + C[Net#b])) ==> (M[Net#b][idx$] == M[Net#a][idx$])
+  assert {:msg "41.15: Action at 3.3 ('anon$0') for actor instance 'pri' might not preserve the channel invariant (#51)"} SqnAct[Net#spl] == R[Net#a];
+  assert {:msg "42.15: Action at 3.3 ('anon$0') for actor instance 'pri' might not preserve the channel invariant (#52)"} SqnAct[Net#pri] == R[Net#b];
+  assert {:msg "43.15: Action at 3.3 ('anon$0') for actor instance 'pri' might not preserve the channel invariant (#53)"} SqnAct[Net#sec] == R[Net#c];
+  assert {:msg "44.15: Action at 3.3 ('anon$0') for actor instance 'pri' might not preserve the channel invariant (#54)"} SqnAct[Net#adj] == R[Net#e];
+  assert {:msg "46.16: Action at 3.3 ('anon$0') for actor instance 'pri' might not preserve the channel invariant (#55)"} (forall i: int :: 
+    (0 <= i) && (i < C[Net#a]) ==> (SqnCh[Net#a][i] == i)
   );
-  assert {:msg "  Action at 3.3 ('anon$0') for actor instance 'pri' might not preserve the channel invariant (#55)"} (forall idx$: int :: 
-    (0 <= idx$) && (idx$ < (R[Net#c] + C[Net#c])) ==> (M[Net#c][idx$] == M[Net#a][idx$])
+  assert {:msg "47.16: Action at 3.3 ('anon$0') for actor instance 'pri' might not preserve the channel invariant (#56)"} (forall i: int :: 
+    (0 <= i) && (i < C[Net#b]) ==> (SqnCh[Net#b][i] == i)
   );
-  assert {:msg "  Action at 3.3 ('anon$0') for actor instance 'pri' might not preserve the channel invariant (#56)"} (forall idx$: int :: 
-    (0 <= idx$) && (idx$ < (R[Net#d] + C[Net#d])) ==> (M[Net#d][idx$] == M[Net#b][idx$])
+  assert {:msg "48.16: Action at 3.3 ('anon$0') for actor instance 'pri' might not preserve the channel invariant (#57)"} (forall i: int :: 
+    (0 <= i) && (i < C[Net#c]) ==> (SqnCh[Net#c][i] == i)
   );
-  assert {:msg "  Action at 3.3 ('anon$0') for actor instance 'pri' might not preserve the channel invariant (#57)"} (forall idx$: int :: 
-    (0 <= idx$) && (idx$ < (R[Net#e] + C[Net#e])) ==> (M[Net#e][idx$] == M[Net#c][idx$])
+  assert {:msg "49.16: Action at 3.3 ('anon$0') for actor instance 'pri' might not preserve the channel invariant (#58)"} (forall i: int :: 
+    (0 <= i) && (i < C[Net#d]) ==> (SqnCh[Net#d][i] == i)
   );
-  assert {:msg "  Action at 3.3 ('anon$0') for actor instance 'pri' might not preserve the channel invariant (#58)"} (forall idx$: int :: 
-    (0 <= idx$) && (idx$ < (R[Net#a] + C[Net#a])) ==> (SqnCh[Net#a][idx$] == idx$)
+  assert {:msg "50.16: Action at 3.3 ('anon$0') for actor instance 'pri' might not preserve the channel invariant (#59)"} (forall i: int :: 
+    (0 <= i) && (i < C[Net#e]) ==> (SqnCh[Net#e][i] == i)
   );
-  assert {:msg "  40.15: Action at 3.3 ('anon$0') for actor instance 'pri' might not preserve the channel invariant (#59)"} SqnAct[Net#spl] == R[Net#a];
-  assert {:msg "  41.15: Action at 3.3 ('anon$0') for actor instance 'pri' might not preserve the channel invariant (#60)"} SqnAct[Net#pri] == R[Net#b];
-  assert {:msg "  42.15: Action at 3.3 ('anon$0') for actor instance 'pri' might not preserve the channel invariant (#61)"} SqnAct[Net#sec] == R[Net#c];
-  assert {:msg "  43.15: Action at 3.3 ('anon$0') for actor instance 'pri' might not preserve the channel invariant (#62)"} SqnAct[Net#adj] == R[Net#e];
-  assert {:msg "  45.16: Action at 3.3 ('anon$0') for actor instance 'pri' might not preserve the channel invariant (#63)"} (forall i: int :: 
-    (0 <= i) && (i < (R[Net#a] + C[Net#a])) ==> (SqnCh[Net#a][i] == i)
+  assert {:msg "51.16: Action at 3.3 ('anon$0') for actor instance 'pri' might not preserve the channel invariant (#60)"} (forall i: int :: 
+    (0 <= i) && (i < C[Net#g]) ==> (SqnCh[Net#g][i] == i)
   );
-  assert {:msg "  46.16: Action at 3.3 ('anon$0') for actor instance 'pri' might not preserve the channel invariant (#64)"} (forall i: int :: 
-    (0 <= i) && (i < (R[Net#b] + C[Net#b])) ==> (SqnCh[Net#b][i] == i)
+  assert {:msg "53.15: Action at 3.3 ('anon$0') for actor instance 'pri' might not preserve the channel invariant (#61)"} (C[Net#f] - R[Net#f]) == 1;
+  assert {:msg "54.15: Action at 3.3 ('anon$0') for actor instance 'pri' might not preserve the channel invariant (#62)"} C[Net#g] == R[Net#e];
+  assert {:msg "55.15: Action at 3.3 ('anon$0') for actor instance 'pri' might not preserve the channel invariant (#63)"} R[Net#e] == M[Net#f][R[Net#f]];
+  assert {:msg "56.16: Action at 3.3 ('anon$0') for actor instance 'pri' might not preserve the channel invariant (#64)"} (forall i: int :: 
+    (0 <= i) && (i < C[Net#g]) ==> (SqnCh[Net#g][i] == i)
   );
-  assert {:msg "  47.16: Action at 3.3 ('anon$0') for actor instance 'pri' might not preserve the channel invariant (#65)"} (forall i: int :: 
-    (0 <= i) && (i < (R[Net#c] + C[Net#c])) ==> (SqnCh[Net#c][i] == i)
-  );
-  assert {:msg "  48.16: Action at 3.3 ('anon$0') for actor instance 'pri' might not preserve the channel invariant (#66)"} (forall i: int :: 
-    (0 <= i) && (i < (R[Net#d] + C[Net#d])) ==> (SqnCh[Net#d][i] == i)
-  );
-  assert {:msg "  49.16: Action at 3.3 ('anon$0') for actor instance 'pri' might not preserve the channel invariant (#67)"} (forall i: int :: 
-    (0 <= i) && (i < (R[Net#e] + C[Net#e])) ==> (SqnCh[Net#e][i] == i)
-  );
-  assert {:msg "  50.16: Action at 3.3 ('anon$0') for actor instance 'pri' might not preserve the channel invariant (#68)"} (forall i: int :: 
-    (0 <= i) && (i < (R[Net#g] + C[Net#g])) ==> (SqnCh[Net#g][i] == i)
-  );
-  assert {:msg "  52.15: Action at 3.3 ('anon$0') for actor instance 'pri' might not preserve the channel invariant (#69)"} C[Net#f] == 1;
-  assert {:msg "  53.15: Action at 3.3 ('anon$0') for actor instance 'pri' might not preserve the channel invariant (#70)"} (R[Net#g] + C[Net#g]) == R[Net#e];
-  assert {:msg "  54.15: Action at 3.3 ('anon$0') for actor instance 'pri' might not preserve the channel invariant (#71)"} R[Net#e] == M[Net#f][R[Net#f]];
-  assert {:msg "  55.16: Action at 3.3 ('anon$0') for actor instance 'pri' might not preserve the channel invariant (#72)"} (forall i: int :: 
-    (0 <= i) && (i < (R[Net#g] + C[Net#g])) ==> (SqnCh[Net#g][i] == i)
-  );
-  if ((0 < R[Net#d]) && (0 < R[Net#e])) {
-    assert {:msg "  57.42: Action at 3.3 ('anon$0') for actor instance 'pri' might not preserve the channel invariant (#73)"} M[Net#d][R[Net#d] - 1] <= M[Net#e][R[Net#e] - 1];
-  }
-  assert {:msg "  58.16: Action at 3.3 ('anon$0') for actor instance 'pri' might not preserve the channel invariant (#74)"} (forall i: int :: 
+  assert {:msg "59.16: Action at 3.3 ('anon$0') for actor instance 'pri' might not preserve the channel invariant (#65)"} (forall i: int :: 
     (0 <= i) && (i < R[Net#e]) ==> (M[Net#g][i] == M[Net#e][i])
   );
+  assert {:msg "Action at 3.3 ('anon$0') for actor instance 'pri' might not preserve the channel invariant (#66)"} R[Net#a] == C[Net#b];
+  assert {:msg "Action at 3.3 ('anon$0') for actor instance 'pri' might not preserve the channel invariant (#67)"} R[Net#a] == C[Net#c];
+  assert {:msg "Action at 3.3 ('anon$0') for actor instance 'pri' might not preserve the channel invariant (#68)"} R[Net#b] == C[Net#d];
+  assert {:msg "Action at 3.3 ('anon$0') for actor instance 'pri' might not preserve the channel invariant (#69)"} R[Net#c] == C[Net#e];
+  assert {:msg "Action at 3.3 ('anon$0') for actor instance 'pri' might not preserve the channel invariant (#70)"} (forall idx$: int :: 
+    (0 <= idx$) && (idx$ < C[Net#b]) ==> (M[Net#b][idx$] == M[Net#a][idx$])
+  );
+  assert {:msg "Action at 3.3 ('anon$0') for actor instance 'pri' might not preserve the channel invariant (#71)"} (forall idx$: int :: 
+    (0 <= idx$) && (idx$ < C[Net#c]) ==> (M[Net#c][idx$] == M[Net#a][idx$])
+  );
+  assert {:msg "Action at 3.3 ('anon$0') for actor instance 'pri' might not preserve the channel invariant (#72)"} (forall idx$: int :: 
+    (0 <= idx$) && (idx$ < C[Net#d]) ==> (M[Net#d][idx$] == M[Net#b][idx$])
+  );
+  assert {:msg "Action at 3.3 ('anon$0') for actor instance 'pri' might not preserve the channel invariant (#73)"} (forall idx$: int :: 
+    (0 <= idx$) && (idx$ < C[Net#e]) ==> (M[Net#e][idx$] == M[Net#c][idx$])
+  );
+  assert {:msg "Action at 3.3 ('anon$0') for actor instance 'pri' might not preserve the channel invariant (#74)"} (forall idx$: int :: 
+    (0 <= idx$) && (idx$ < C[Net#a]) ==> (SqnCh[Net#a][idx$] == idx$)
+  );
 }
-procedure Net#anon$3#Rep#anon$0#10()
-  modifies C, R, M, St, SqnCh, SqnAct;
+procedure Net##Rep#anon$0#10()
+  modifies C, R, M, I, St, SqnCh, SqnAct;
 {
   var St#next: State;
   var in#i: int;
-  assume L[Net#a] == (1 * Base#L);
-  assume 0 <= R[Net#a];
-  assume 0 <= C[Net#a];
-  assume (R[Net#a] + C[Net#a]) <= L[Net#a];
-  assume 0 <= R[Net#b];
-  assume 0 <= C[Net#b];
-  assume 0 <= R[Net#c];
-  assume 0 <= C[Net#c];
-  assume 0 <= R[Net#d];
-  assume 0 <= C[Net#d];
-  assume 0 <= R[Net#e];
-  assume 0 <= C[Net#e];
-  assume 0 <= R[Net#f];
-  assume 0 <= C[Net#f];
-  assume 0 <= R[Net#g];
-  assume 0 <= C[Net#g];
-  assume R[Net#g] == 0;
-  assume R[Net#a] == (R[Net#b] + C[Net#b]);
-  assume R[Net#a] == (R[Net#c] + C[Net#c]);
-  assume R[Net#b] == (R[Net#d] + C[Net#d]);
-  assume R[Net#c] == (R[Net#e] + C[Net#e]);
-  assume (forall idx$: int :: 
-    (0 <= idx$) && (idx$ < (R[Net#b] + C[Net#b])) ==> (M[Net#b][idx$] == M[Net#a][idx$])
-  );
-  assume (forall idx$: int :: 
-    (0 <= idx$) && (idx$ < (R[Net#c] + C[Net#c])) ==> (M[Net#c][idx$] == M[Net#a][idx$])
-  );
-  assume (forall idx$: int :: 
-    (0 <= idx$) && (idx$ < (R[Net#d] + C[Net#d])) ==> (M[Net#d][idx$] == M[Net#b][idx$])
-  );
-  assume (forall idx$: int :: 
-    (0 <= idx$) && (idx$ < (R[Net#e] + C[Net#e])) ==> (M[Net#e][idx$] == M[Net#c][idx$])
-  );
-  assume (forall idx$: int :: 
-    (0 <= idx$) && (idx$ < (R[Net#a] + C[Net#a])) ==> (SqnCh[Net#a][idx$] == idx$)
-  );
+  assume 0 <= I[Net#a];
+  assume I[Net#a] <= R[Net#a];
+  assume R[Net#a] <= C[Net#a];
+  assume 0 <= I[Net#b];
+  assume I[Net#b] <= R[Net#b];
+  assume R[Net#b] <= C[Net#b];
+  assume 0 <= I[Net#c];
+  assume I[Net#c] <= R[Net#c];
+  assume R[Net#c] <= C[Net#c];
+  assume 0 <= I[Net#d];
+  assume I[Net#d] <= R[Net#d];
+  assume R[Net#d] <= C[Net#d];
+  assume 0 <= I[Net#e];
+  assume I[Net#e] <= R[Net#e];
+  assume R[Net#e] <= C[Net#e];
+  assume 0 <= I[Net#f];
+  assume I[Net#f] <= R[Net#f];
+  assume R[Net#f] <= C[Net#f];
+  assume 0 <= I[Net#g];
+  assume I[Net#g] <= R[Net#g];
+  assume R[Net#g] <= C[Net#g];
+  assume I[Net#g] == R[Net#g];
   assume SqnAct[Net#spl] == R[Net#a];
   assume SqnAct[Net#pri] == R[Net#b];
   assume SqnAct[Net#sec] == R[Net#c];
   assume SqnAct[Net#adj] == R[Net#e];
   assume (forall i: int :: 
-    (0 <= i) && (i < (R[Net#a] + C[Net#a])) ==> (SqnCh[Net#a][i] == i)
+    (0 <= i) && (i < C[Net#a]) ==> (SqnCh[Net#a][i] == i)
   );
   assume (forall i: int :: 
-    (0 <= i) && (i < (R[Net#b] + C[Net#b])) ==> (SqnCh[Net#b][i] == i)
+    (0 <= i) && (i < C[Net#b]) ==> (SqnCh[Net#b][i] == i)
   );
   assume (forall i: int :: 
-    (0 <= i) && (i < (R[Net#c] + C[Net#c])) ==> (SqnCh[Net#c][i] == i)
+    (0 <= i) && (i < C[Net#c]) ==> (SqnCh[Net#c][i] == i)
   );
   assume (forall i: int :: 
-    (0 <= i) && (i < (R[Net#d] + C[Net#d])) ==> (SqnCh[Net#d][i] == i)
+    (0 <= i) && (i < C[Net#d]) ==> (SqnCh[Net#d][i] == i)
   );
   assume (forall i: int :: 
-    (0 <= i) && (i < (R[Net#e] + C[Net#e])) ==> (SqnCh[Net#e][i] == i)
+    (0 <= i) && (i < C[Net#e]) ==> (SqnCh[Net#e][i] == i)
   );
   assume (forall i: int :: 
-    (0 <= i) && (i < (R[Net#g] + C[Net#g])) ==> (SqnCh[Net#g][i] == i)
+    (0 <= i) && (i < C[Net#g]) ==> (SqnCh[Net#g][i] == i)
   );
-  assume C[Net#f] == 1;
-  assume (R[Net#g] + C[Net#g]) == R[Net#e];
+  assume (C[Net#f] - R[Net#f]) == 1;
+  assume C[Net#g] == R[Net#e];
   assume R[Net#e] == M[Net#f][R[Net#f]];
   assume (forall i: int :: 
-    (0 <= i) && (i < (R[Net#g] + C[Net#g])) ==> (SqnCh[Net#g][i] == i)
+    (0 <= i) && (i < C[Net#g]) ==> (SqnCh[Net#g][i] == i)
   );
-  if ((0 < R[Net#d]) && (0 < R[Net#e])) {
-    assume M[Net#d][R[Net#d] - 1] <= M[Net#e][R[Net#e] - 1];
-  }
   assume (forall i: int :: 
     (0 <= i) && (i < R[Net#e]) ==> (M[Net#g][i] == M[Net#e][i])
   );
+  assume R[Net#a] == C[Net#b];
+  assume R[Net#a] == C[Net#c];
+  assume R[Net#b] == C[Net#d];
+  assume R[Net#c] == C[Net#e];
+  assume (forall idx$: int :: 
+    (0 <= idx$) && (idx$ < C[Net#b]) ==> (M[Net#b][idx$] == M[Net#a][idx$])
+  );
+  assume (forall idx$: int :: 
+    (0 <= idx$) && (idx$ < C[Net#c]) ==> (M[Net#c][idx$] == M[Net#a][idx$])
+  );
+  assume (forall idx$: int :: 
+    (0 <= idx$) && (idx$ < C[Net#d]) ==> (M[Net#d][idx$] == M[Net#b][idx$])
+  );
+  assume (forall idx$: int :: 
+    (0 <= idx$) && (idx$ < C[Net#e]) ==> (M[Net#e][idx$] == M[Net#c][idx$])
+  );
+  assume (forall idx$: int :: 
+    (0 <= idx$) && (idx$ < C[Net#a]) ==> (SqnCh[Net#a][idx$] == idx$)
+  );
   assume true;
-  assume 1 <= C[Net#c];
+  assume 1 <= (C[Net#c] - R[Net#c]);
   in#i := M[Net#c][R[Net#c]];
   R[Net#c] := R[Net#c] + 1;
-  C[Net#c] := C[Net#c] - 1;
-  M[Net#e][R[Net#e] + C[Net#e]] := in#i;
-  SqnCh[Net#e][R[Net#e] + C[Net#e]] := SqnAct[Net#sec];
+  M[Net#e][C[Net#e]] := in#i;
+  SqnCh[Net#e][C[Net#e]] := SqnAct[Net#sec];
   C[Net#e] := C[Net#e] + 1;
   SqnAct[Net#sec] := SqnAct[Net#sec] + 1;
-  assert {:msg "  Action at 3.3 ('anon$0') for actor instance 'sec' might not preserve the channel invariant (#75)"} R[Net#a] == (R[Net#b] + C[Net#b]);
-  assert {:msg "  Action at 3.3 ('anon$0') for actor instance 'sec' might not preserve the channel invariant (#76)"} R[Net#a] == (R[Net#c] + C[Net#c]);
-  assert {:msg "  Action at 3.3 ('anon$0') for actor instance 'sec' might not preserve the channel invariant (#77)"} R[Net#b] == (R[Net#d] + C[Net#d]);
-  assert {:msg "  Action at 3.3 ('anon$0') for actor instance 'sec' might not preserve the channel invariant (#78)"} R[Net#c] == (R[Net#e] + C[Net#e]);
-  assert {:msg "  Action at 3.3 ('anon$0') for actor instance 'sec' might not preserve the channel invariant (#79)"} (forall idx$: int :: 
-    (0 <= idx$) && (idx$ < (R[Net#b] + C[Net#b])) ==> (M[Net#b][idx$] == M[Net#a][idx$])
+  assert {:msg "41.15: Action at 3.3 ('anon$0') for actor instance 'sec' might not preserve the channel invariant (#75)"} SqnAct[Net#spl] == R[Net#a];
+  assert {:msg "42.15: Action at 3.3 ('anon$0') for actor instance 'sec' might not preserve the channel invariant (#76)"} SqnAct[Net#pri] == R[Net#b];
+  assert {:msg "43.15: Action at 3.3 ('anon$0') for actor instance 'sec' might not preserve the channel invariant (#77)"} SqnAct[Net#sec] == R[Net#c];
+  assert {:msg "44.15: Action at 3.3 ('anon$0') for actor instance 'sec' might not preserve the channel invariant (#78)"} SqnAct[Net#adj] == R[Net#e];
+  assert {:msg "46.16: Action at 3.3 ('anon$0') for actor instance 'sec' might not preserve the channel invariant (#79)"} (forall i: int :: 
+    (0 <= i) && (i < C[Net#a]) ==> (SqnCh[Net#a][i] == i)
   );
-  assert {:msg "  Action at 3.3 ('anon$0') for actor instance 'sec' might not preserve the channel invariant (#80)"} (forall idx$: int :: 
-    (0 <= idx$) && (idx$ < (R[Net#c] + C[Net#c])) ==> (M[Net#c][idx$] == M[Net#a][idx$])
+  assert {:msg "47.16: Action at 3.3 ('anon$0') for actor instance 'sec' might not preserve the channel invariant (#80)"} (forall i: int :: 
+    (0 <= i) && (i < C[Net#b]) ==> (SqnCh[Net#b][i] == i)
   );
-  assert {:msg "  Action at 3.3 ('anon$0') for actor instance 'sec' might not preserve the channel invariant (#81)"} (forall idx$: int :: 
-    (0 <= idx$) && (idx$ < (R[Net#d] + C[Net#d])) ==> (M[Net#d][idx$] == M[Net#b][idx$])
+  assert {:msg "48.16: Action at 3.3 ('anon$0') for actor instance 'sec' might not preserve the channel invariant (#81)"} (forall i: int :: 
+    (0 <= i) && (i < C[Net#c]) ==> (SqnCh[Net#c][i] == i)
   );
-  assert {:msg "  Action at 3.3 ('anon$0') for actor instance 'sec' might not preserve the channel invariant (#82)"} (forall idx$: int :: 
-    (0 <= idx$) && (idx$ < (R[Net#e] + C[Net#e])) ==> (M[Net#e][idx$] == M[Net#c][idx$])
+  assert {:msg "49.16: Action at 3.3 ('anon$0') for actor instance 'sec' might not preserve the channel invariant (#82)"} (forall i: int :: 
+    (0 <= i) && (i < C[Net#d]) ==> (SqnCh[Net#d][i] == i)
   );
-  assert {:msg "  Action at 3.3 ('anon$0') for actor instance 'sec' might not preserve the channel invariant (#83)"} (forall idx$: int :: 
-    (0 <= idx$) && (idx$ < (R[Net#a] + C[Net#a])) ==> (SqnCh[Net#a][idx$] == idx$)
+  assert {:msg "50.16: Action at 3.3 ('anon$0') for actor instance 'sec' might not preserve the channel invariant (#83)"} (forall i: int :: 
+    (0 <= i) && (i < C[Net#e]) ==> (SqnCh[Net#e][i] == i)
   );
-  assert {:msg "  40.15: Action at 3.3 ('anon$0') for actor instance 'sec' might not preserve the channel invariant (#84)"} SqnAct[Net#spl] == R[Net#a];
-  assert {:msg "  41.15: Action at 3.3 ('anon$0') for actor instance 'sec' might not preserve the channel invariant (#85)"} SqnAct[Net#pri] == R[Net#b];
-  assert {:msg "  42.15: Action at 3.3 ('anon$0') for actor instance 'sec' might not preserve the channel invariant (#86)"} SqnAct[Net#sec] == R[Net#c];
-  assert {:msg "  43.15: Action at 3.3 ('anon$0') for actor instance 'sec' might not preserve the channel invariant (#87)"} SqnAct[Net#adj] == R[Net#e];
-  assert {:msg "  45.16: Action at 3.3 ('anon$0') for actor instance 'sec' might not preserve the channel invariant (#88)"} (forall i: int :: 
-    (0 <= i) && (i < (R[Net#a] + C[Net#a])) ==> (SqnCh[Net#a][i] == i)
+  assert {:msg "51.16: Action at 3.3 ('anon$0') for actor instance 'sec' might not preserve the channel invariant (#84)"} (forall i: int :: 
+    (0 <= i) && (i < C[Net#g]) ==> (SqnCh[Net#g][i] == i)
   );
-  assert {:msg "  46.16: Action at 3.3 ('anon$0') for actor instance 'sec' might not preserve the channel invariant (#89)"} (forall i: int :: 
-    (0 <= i) && (i < (R[Net#b] + C[Net#b])) ==> (SqnCh[Net#b][i] == i)
+  assert {:msg "53.15: Action at 3.3 ('anon$0') for actor instance 'sec' might not preserve the channel invariant (#85)"} (C[Net#f] - R[Net#f]) == 1;
+  assert {:msg "54.15: Action at 3.3 ('anon$0') for actor instance 'sec' might not preserve the channel invariant (#86)"} C[Net#g] == R[Net#e];
+  assert {:msg "55.15: Action at 3.3 ('anon$0') for actor instance 'sec' might not preserve the channel invariant (#87)"} R[Net#e] == M[Net#f][R[Net#f]];
+  assert {:msg "56.16: Action at 3.3 ('anon$0') for actor instance 'sec' might not preserve the channel invariant (#88)"} (forall i: int :: 
+    (0 <= i) && (i < C[Net#g]) ==> (SqnCh[Net#g][i] == i)
   );
-  assert {:msg "  47.16: Action at 3.3 ('anon$0') for actor instance 'sec' might not preserve the channel invariant (#90)"} (forall i: int :: 
-    (0 <= i) && (i < (R[Net#c] + C[Net#c])) ==> (SqnCh[Net#c][i] == i)
-  );
-  assert {:msg "  48.16: Action at 3.3 ('anon$0') for actor instance 'sec' might not preserve the channel invariant (#91)"} (forall i: int :: 
-    (0 <= i) && (i < (R[Net#d] + C[Net#d])) ==> (SqnCh[Net#d][i] == i)
-  );
-  assert {:msg "  49.16: Action at 3.3 ('anon$0') for actor instance 'sec' might not preserve the channel invariant (#92)"} (forall i: int :: 
-    (0 <= i) && (i < (R[Net#e] + C[Net#e])) ==> (SqnCh[Net#e][i] == i)
-  );
-  assert {:msg "  50.16: Action at 3.3 ('anon$0') for actor instance 'sec' might not preserve the channel invariant (#93)"} (forall i: int :: 
-    (0 <= i) && (i < (R[Net#g] + C[Net#g])) ==> (SqnCh[Net#g][i] == i)
-  );
-  assert {:msg "  52.15: Action at 3.3 ('anon$0') for actor instance 'sec' might not preserve the channel invariant (#94)"} C[Net#f] == 1;
-  assert {:msg "  53.15: Action at 3.3 ('anon$0') for actor instance 'sec' might not preserve the channel invariant (#95)"} (R[Net#g] + C[Net#g]) == R[Net#e];
-  assert {:msg "  54.15: Action at 3.3 ('anon$0') for actor instance 'sec' might not preserve the channel invariant (#96)"} R[Net#e] == M[Net#f][R[Net#f]];
-  assert {:msg "  55.16: Action at 3.3 ('anon$0') for actor instance 'sec' might not preserve the channel invariant (#97)"} (forall i: int :: 
-    (0 <= i) && (i < (R[Net#g] + C[Net#g])) ==> (SqnCh[Net#g][i] == i)
-  );
-  if ((0 < R[Net#d]) && (0 < R[Net#e])) {
-    assert {:msg "  57.42: Action at 3.3 ('anon$0') for actor instance 'sec' might not preserve the channel invariant (#98)"} M[Net#d][R[Net#d] - 1] <= M[Net#e][R[Net#e] - 1];
-  }
-  assert {:msg "  58.16: Action at 3.3 ('anon$0') for actor instance 'sec' might not preserve the channel invariant (#99)"} (forall i: int :: 
+  assert {:msg "59.16: Action at 3.3 ('anon$0') for actor instance 'sec' might not preserve the channel invariant (#89)"} (forall i: int :: 
     (0 <= i) && (i < R[Net#e]) ==> (M[Net#g][i] == M[Net#e][i])
   );
+  assert {:msg "Action at 3.3 ('anon$0') for actor instance 'sec' might not preserve the channel invariant (#90)"} R[Net#a] == C[Net#b];
+  assert {:msg "Action at 3.3 ('anon$0') for actor instance 'sec' might not preserve the channel invariant (#91)"} R[Net#a] == C[Net#c];
+  assert {:msg "Action at 3.3 ('anon$0') for actor instance 'sec' might not preserve the channel invariant (#92)"} R[Net#b] == C[Net#d];
+  assert {:msg "Action at 3.3 ('anon$0') for actor instance 'sec' might not preserve the channel invariant (#93)"} R[Net#c] == C[Net#e];
+  assert {:msg "Action at 3.3 ('anon$0') for actor instance 'sec' might not preserve the channel invariant (#94)"} (forall idx$: int :: 
+    (0 <= idx$) && (idx$ < C[Net#b]) ==> (M[Net#b][idx$] == M[Net#a][idx$])
+  );
+  assert {:msg "Action at 3.3 ('anon$0') for actor instance 'sec' might not preserve the channel invariant (#95)"} (forall idx$: int :: 
+    (0 <= idx$) && (idx$ < C[Net#c]) ==> (M[Net#c][idx$] == M[Net#a][idx$])
+  );
+  assert {:msg "Action at 3.3 ('anon$0') for actor instance 'sec' might not preserve the channel invariant (#96)"} (forall idx$: int :: 
+    (0 <= idx$) && (idx$ < C[Net#d]) ==> (M[Net#d][idx$] == M[Net#b][idx$])
+  );
+  assert {:msg "Action at 3.3 ('anon$0') for actor instance 'sec' might not preserve the channel invariant (#97)"} (forall idx$: int :: 
+    (0 <= idx$) && (idx$ < C[Net#e]) ==> (M[Net#e][idx$] == M[Net#c][idx$])
+  );
+  assert {:msg "Action at 3.3 ('anon$0') for actor instance 'sec' might not preserve the channel invariant (#98)"} (forall idx$: int :: 
+    (0 <= idx$) && (idx$ < C[Net#a]) ==> (SqnCh[Net#a][idx$] == idx$)
+  );
 }
-procedure Net#anon$3#Adjudicator#readoff#11()
-  modifies C, R, M, St, SqnCh, SqnAct;
+procedure Net##Adjudicator#readoff#11()
+  modifies C, R, M, I, St, SqnCh, SqnAct;
 {
   var St#next: State;
   var x1#i: int;
   var c_in#c: int;
-  assume L[Net#a] == (1 * Base#L);
-  assume 0 <= R[Net#a];
-  assume 0 <= C[Net#a];
-  assume (R[Net#a] + C[Net#a]) <= L[Net#a];
-  assume 0 <= R[Net#b];
-  assume 0 <= C[Net#b];
-  assume 0 <= R[Net#c];
-  assume 0 <= C[Net#c];
-  assume 0 <= R[Net#d];
-  assume 0 <= C[Net#d];
-  assume 0 <= R[Net#e];
-  assume 0 <= C[Net#e];
-  assume 0 <= R[Net#f];
-  assume 0 <= C[Net#f];
-  assume 0 <= R[Net#g];
-  assume 0 <= C[Net#g];
-  assume R[Net#g] == 0;
-  assume R[Net#a] == (R[Net#b] + C[Net#b]);
-  assume R[Net#a] == (R[Net#c] + C[Net#c]);
-  assume R[Net#b] == (R[Net#d] + C[Net#d]);
-  assume R[Net#c] == (R[Net#e] + C[Net#e]);
-  assume (forall idx$: int :: 
-    (0 <= idx$) && (idx$ < (R[Net#b] + C[Net#b])) ==> (M[Net#b][idx$] == M[Net#a][idx$])
-  );
-  assume (forall idx$: int :: 
-    (0 <= idx$) && (idx$ < (R[Net#c] + C[Net#c])) ==> (M[Net#c][idx$] == M[Net#a][idx$])
-  );
-  assume (forall idx$: int :: 
-    (0 <= idx$) && (idx$ < (R[Net#d] + C[Net#d])) ==> (M[Net#d][idx$] == M[Net#b][idx$])
-  );
-  assume (forall idx$: int :: 
-    (0 <= idx$) && (idx$ < (R[Net#e] + C[Net#e])) ==> (M[Net#e][idx$] == M[Net#c][idx$])
-  );
-  assume (forall idx$: int :: 
-    (0 <= idx$) && (idx$ < (R[Net#a] + C[Net#a])) ==> (SqnCh[Net#a][idx$] == idx$)
-  );
+  assume 0 <= I[Net#a];
+  assume I[Net#a] <= R[Net#a];
+  assume R[Net#a] <= C[Net#a];
+  assume 0 <= I[Net#b];
+  assume I[Net#b] <= R[Net#b];
+  assume R[Net#b] <= C[Net#b];
+  assume 0 <= I[Net#c];
+  assume I[Net#c] <= R[Net#c];
+  assume R[Net#c] <= C[Net#c];
+  assume 0 <= I[Net#d];
+  assume I[Net#d] <= R[Net#d];
+  assume R[Net#d] <= C[Net#d];
+  assume 0 <= I[Net#e];
+  assume I[Net#e] <= R[Net#e];
+  assume R[Net#e] <= C[Net#e];
+  assume 0 <= I[Net#f];
+  assume I[Net#f] <= R[Net#f];
+  assume R[Net#f] <= C[Net#f];
+  assume 0 <= I[Net#g];
+  assume I[Net#g] <= R[Net#g];
+  assume R[Net#g] <= C[Net#g];
+  assume I[Net#g] == R[Net#g];
   assume SqnAct[Net#spl] == R[Net#a];
   assume SqnAct[Net#pri] == R[Net#b];
   assume SqnAct[Net#sec] == R[Net#c];
   assume SqnAct[Net#adj] == R[Net#e];
   assume (forall i: int :: 
-    (0 <= i) && (i < (R[Net#a] + C[Net#a])) ==> (SqnCh[Net#a][i] == i)
+    (0 <= i) && (i < C[Net#a]) ==> (SqnCh[Net#a][i] == i)
   );
   assume (forall i: int :: 
-    (0 <= i) && (i < (R[Net#b] + C[Net#b])) ==> (SqnCh[Net#b][i] == i)
+    (0 <= i) && (i < C[Net#b]) ==> (SqnCh[Net#b][i] == i)
   );
   assume (forall i: int :: 
-    (0 <= i) && (i < (R[Net#c] + C[Net#c])) ==> (SqnCh[Net#c][i] == i)
+    (0 <= i) && (i < C[Net#c]) ==> (SqnCh[Net#c][i] == i)
   );
   assume (forall i: int :: 
-    (0 <= i) && (i < (R[Net#d] + C[Net#d])) ==> (SqnCh[Net#d][i] == i)
+    (0 <= i) && (i < C[Net#d]) ==> (SqnCh[Net#d][i] == i)
   );
   assume (forall i: int :: 
-    (0 <= i) && (i < (R[Net#e] + C[Net#e])) ==> (SqnCh[Net#e][i] == i)
+    (0 <= i) && (i < C[Net#e]) ==> (SqnCh[Net#e][i] == i)
   );
   assume (forall i: int :: 
-    (0 <= i) && (i < (R[Net#g] + C[Net#g])) ==> (SqnCh[Net#g][i] == i)
+    (0 <= i) && (i < C[Net#g]) ==> (SqnCh[Net#g][i] == i)
   );
-  assume C[Net#f] == 1;
-  assume (R[Net#g] + C[Net#g]) == R[Net#e];
+  assume (C[Net#f] - R[Net#f]) == 1;
+  assume C[Net#g] == R[Net#e];
   assume R[Net#e] == M[Net#f][R[Net#f]];
   assume (forall i: int :: 
-    (0 <= i) && (i < (R[Net#g] + C[Net#g])) ==> (SqnCh[Net#g][i] == i)
+    (0 <= i) && (i < C[Net#g]) ==> (SqnCh[Net#g][i] == i)
   );
-  if ((0 < R[Net#d]) && (0 < R[Net#e])) {
-    assume M[Net#d][R[Net#d] - 1] <= M[Net#e][R[Net#e] - 1];
-  }
   assume (forall i: int :: 
     (0 <= i) && (i < R[Net#e]) ==> (M[Net#g][i] == M[Net#e][i])
+  );
+  assume R[Net#a] == C[Net#b];
+  assume R[Net#a] == C[Net#c];
+  assume R[Net#b] == C[Net#d];
+  assume R[Net#c] == C[Net#e];
+  assume (forall idx$: int :: 
+    (0 <= idx$) && (idx$ < C[Net#b]) ==> (M[Net#b][idx$] == M[Net#a][idx$])
+  );
+  assume (forall idx$: int :: 
+    (0 <= idx$) && (idx$ < C[Net#c]) ==> (M[Net#c][idx$] == M[Net#a][idx$])
+  );
+  assume (forall idx$: int :: 
+    (0 <= idx$) && (idx$ < C[Net#d]) ==> (M[Net#d][idx$] == M[Net#b][idx$])
+  );
+  assume (forall idx$: int :: 
+    (0 <= idx$) && (idx$ < C[Net#e]) ==> (M[Net#e][idx$] == M[Net#c][idx$])
+  );
+  assume (forall idx$: int :: 
+    (0 <= idx$) && (idx$ < C[Net#a]) ==> (SqnCh[Net#a][idx$] == idx$)
   );
   assume SqnCh[Net#d][R[Net#d] - 0] < M[Net#f][R[Net#f] - 0];
   assume true;
-  assume (1 <= C[Net#d]) && (1 <= C[Net#f]) && (SqnCh[Net#d][R[Net#d] - 0] < M[Net#f][R[Net#f] - 0]);
+  assume (1 <= (C[Net#d] - R[Net#d])) && (1 <= (C[Net#f] - R[Net#f])) && (SqnCh[Net#d][R[Net#d] - 0] < M[Net#f][R[Net#f] - 0]);
   x1#i := M[Net#d][R[Net#d]];
   R[Net#d] := R[Net#d] + 1;
-  C[Net#d] := C[Net#d] - 1;
   c_in#c := M[Net#f][R[Net#f]];
   R[Net#f] := R[Net#f] + 1;
-  C[Net#f] := C[Net#f] - 1;
-  M[Net#f][R[Net#f] + C[Net#f]] := c_in#c;
-  SqnCh[Net#f][R[Net#f] + C[Net#f]] := SqnAct[Net#adj];
+  M[Net#f][C[Net#f]] := c_in#c;
+  SqnCh[Net#f][C[Net#f]] := SqnAct[Net#adj];
   C[Net#f] := C[Net#f] + 1;
-  assert {:msg "  Action at 20.3 ('readoff') for actor instance 'adj' might not preserve the channel invariant (#100)"} R[Net#a] == (R[Net#b] + C[Net#b]);
-  assert {:msg "  Action at 20.3 ('readoff') for actor instance 'adj' might not preserve the channel invariant (#101)"} R[Net#a] == (R[Net#c] + C[Net#c]);
-  assert {:msg "  Action at 20.3 ('readoff') for actor instance 'adj' might not preserve the channel invariant (#102)"} R[Net#b] == (R[Net#d] + C[Net#d]);
-  assert {:msg "  Action at 20.3 ('readoff') for actor instance 'adj' might not preserve the channel invariant (#103)"} R[Net#c] == (R[Net#e] + C[Net#e]);
-  assert {:msg "  Action at 20.3 ('readoff') for actor instance 'adj' might not preserve the channel invariant (#104)"} (forall idx$: int :: 
-    (0 <= idx$) && (idx$ < (R[Net#b] + C[Net#b])) ==> (M[Net#b][idx$] == M[Net#a][idx$])
+  assert {:msg "41.15: Action at 20.3 ('readoff') for actor instance 'adj' might not preserve the channel invariant (#99)"} SqnAct[Net#spl] == R[Net#a];
+  assert {:msg "42.15: Action at 20.3 ('readoff') for actor instance 'adj' might not preserve the channel invariant (#100)"} SqnAct[Net#pri] == R[Net#b];
+  assert {:msg "43.15: Action at 20.3 ('readoff') for actor instance 'adj' might not preserve the channel invariant (#101)"} SqnAct[Net#sec] == R[Net#c];
+  assert {:msg "44.15: Action at 20.3 ('readoff') for actor instance 'adj' might not preserve the channel invariant (#102)"} SqnAct[Net#adj] == R[Net#e];
+  assert {:msg "46.16: Action at 20.3 ('readoff') for actor instance 'adj' might not preserve the channel invariant (#103)"} (forall i: int :: 
+    (0 <= i) && (i < C[Net#a]) ==> (SqnCh[Net#a][i] == i)
   );
-  assert {:msg "  Action at 20.3 ('readoff') for actor instance 'adj' might not preserve the channel invariant (#105)"} (forall idx$: int :: 
-    (0 <= idx$) && (idx$ < (R[Net#c] + C[Net#c])) ==> (M[Net#c][idx$] == M[Net#a][idx$])
+  assert {:msg "47.16: Action at 20.3 ('readoff') for actor instance 'adj' might not preserve the channel invariant (#104)"} (forall i: int :: 
+    (0 <= i) && (i < C[Net#b]) ==> (SqnCh[Net#b][i] == i)
   );
-  assert {:msg "  Action at 20.3 ('readoff') for actor instance 'adj' might not preserve the channel invariant (#106)"} (forall idx$: int :: 
-    (0 <= idx$) && (idx$ < (R[Net#d] + C[Net#d])) ==> (M[Net#d][idx$] == M[Net#b][idx$])
+  assert {:msg "48.16: Action at 20.3 ('readoff') for actor instance 'adj' might not preserve the channel invariant (#105)"} (forall i: int :: 
+    (0 <= i) && (i < C[Net#c]) ==> (SqnCh[Net#c][i] == i)
   );
-  assert {:msg "  Action at 20.3 ('readoff') for actor instance 'adj' might not preserve the channel invariant (#107)"} (forall idx$: int :: 
-    (0 <= idx$) && (idx$ < (R[Net#e] + C[Net#e])) ==> (M[Net#e][idx$] == M[Net#c][idx$])
+  assert {:msg "49.16: Action at 20.3 ('readoff') for actor instance 'adj' might not preserve the channel invariant (#106)"} (forall i: int :: 
+    (0 <= i) && (i < C[Net#d]) ==> (SqnCh[Net#d][i] == i)
   );
-  assert {:msg "  Action at 20.3 ('readoff') for actor instance 'adj' might not preserve the channel invariant (#108)"} (forall idx$: int :: 
-    (0 <= idx$) && (idx$ < (R[Net#a] + C[Net#a])) ==> (SqnCh[Net#a][idx$] == idx$)
+  assert {:msg "50.16: Action at 20.3 ('readoff') for actor instance 'adj' might not preserve the channel invariant (#107)"} (forall i: int :: 
+    (0 <= i) && (i < C[Net#e]) ==> (SqnCh[Net#e][i] == i)
   );
-  assert {:msg "  40.15: Action at 20.3 ('readoff') for actor instance 'adj' might not preserve the channel invariant (#109)"} SqnAct[Net#spl] == R[Net#a];
-  assert {:msg "  41.15: Action at 20.3 ('readoff') for actor instance 'adj' might not preserve the channel invariant (#110)"} SqnAct[Net#pri] == R[Net#b];
-  assert {:msg "  42.15: Action at 20.3 ('readoff') for actor instance 'adj' might not preserve the channel invariant (#111)"} SqnAct[Net#sec] == R[Net#c];
-  assert {:msg "  43.15: Action at 20.3 ('readoff') for actor instance 'adj' might not preserve the channel invariant (#112)"} SqnAct[Net#adj] == R[Net#e];
-  assert {:msg "  45.16: Action at 20.3 ('readoff') for actor instance 'adj' might not preserve the channel invariant (#113)"} (forall i: int :: 
-    (0 <= i) && (i < (R[Net#a] + C[Net#a])) ==> (SqnCh[Net#a][i] == i)
+  assert {:msg "51.16: Action at 20.3 ('readoff') for actor instance 'adj' might not preserve the channel invariant (#108)"} (forall i: int :: 
+    (0 <= i) && (i < C[Net#g]) ==> (SqnCh[Net#g][i] == i)
   );
-  assert {:msg "  46.16: Action at 20.3 ('readoff') for actor instance 'adj' might not preserve the channel invariant (#114)"} (forall i: int :: 
-    (0 <= i) && (i < (R[Net#b] + C[Net#b])) ==> (SqnCh[Net#b][i] == i)
+  assert {:msg "53.15: Action at 20.3 ('readoff') for actor instance 'adj' might not preserve the channel invariant (#109)"} (C[Net#f] - R[Net#f]) == 1;
+  assert {:msg "54.15: Action at 20.3 ('readoff') for actor instance 'adj' might not preserve the channel invariant (#110)"} C[Net#g] == R[Net#e];
+  assert {:msg "55.15: Action at 20.3 ('readoff') for actor instance 'adj' might not preserve the channel invariant (#111)"} R[Net#e] == M[Net#f][R[Net#f]];
+  assert {:msg "56.16: Action at 20.3 ('readoff') for actor instance 'adj' might not preserve the channel invariant (#112)"} (forall i: int :: 
+    (0 <= i) && (i < C[Net#g]) ==> (SqnCh[Net#g][i] == i)
   );
-  assert {:msg "  47.16: Action at 20.3 ('readoff') for actor instance 'adj' might not preserve the channel invariant (#115)"} (forall i: int :: 
-    (0 <= i) && (i < (R[Net#c] + C[Net#c])) ==> (SqnCh[Net#c][i] == i)
-  );
-  assert {:msg "  48.16: Action at 20.3 ('readoff') for actor instance 'adj' might not preserve the channel invariant (#116)"} (forall i: int :: 
-    (0 <= i) && (i < (R[Net#d] + C[Net#d])) ==> (SqnCh[Net#d][i] == i)
-  );
-  assert {:msg "  49.16: Action at 20.3 ('readoff') for actor instance 'adj' might not preserve the channel invariant (#117)"} (forall i: int :: 
-    (0 <= i) && (i < (R[Net#e] + C[Net#e])) ==> (SqnCh[Net#e][i] == i)
-  );
-  assert {:msg "  50.16: Action at 20.3 ('readoff') for actor instance 'adj' might not preserve the channel invariant (#118)"} (forall i: int :: 
-    (0 <= i) && (i < (R[Net#g] + C[Net#g])) ==> (SqnCh[Net#g][i] == i)
-  );
-  assert {:msg "  52.15: Action at 20.3 ('readoff') for actor instance 'adj' might not preserve the channel invariant (#119)"} C[Net#f] == 1;
-  assert {:msg "  53.15: Action at 20.3 ('readoff') for actor instance 'adj' might not preserve the channel invariant (#120)"} (R[Net#g] + C[Net#g]) == R[Net#e];
-  assert {:msg "  54.15: Action at 20.3 ('readoff') for actor instance 'adj' might not preserve the channel invariant (#121)"} R[Net#e] == M[Net#f][R[Net#f]];
-  assert {:msg "  55.16: Action at 20.3 ('readoff') for actor instance 'adj' might not preserve the channel invariant (#122)"} (forall i: int :: 
-    (0 <= i) && (i < (R[Net#g] + C[Net#g])) ==> (SqnCh[Net#g][i] == i)
-  );
-  if ((0 < R[Net#d]) && (0 < R[Net#e])) {
-    assert {:msg "  57.42: Action at 20.3 ('readoff') for actor instance 'adj' might not preserve the channel invariant (#123)"} M[Net#d][R[Net#d] - 1] <= M[Net#e][R[Net#e] - 1];
-  }
-  assert {:msg "  58.16: Action at 20.3 ('readoff') for actor instance 'adj' might not preserve the channel invariant (#124)"} (forall i: int :: 
+  assert {:msg "59.16: Action at 20.3 ('readoff') for actor instance 'adj' might not preserve the channel invariant (#113)"} (forall i: int :: 
     (0 <= i) && (i < R[Net#e]) ==> (M[Net#g][i] == M[Net#e][i])
   );
+  assert {:msg "Action at 20.3 ('readoff') for actor instance 'adj' might not preserve the channel invariant (#114)"} R[Net#a] == C[Net#b];
+  assert {:msg "Action at 20.3 ('readoff') for actor instance 'adj' might not preserve the channel invariant (#115)"} R[Net#a] == C[Net#c];
+  assert {:msg "Action at 20.3 ('readoff') for actor instance 'adj' might not preserve the channel invariant (#116)"} R[Net#b] == C[Net#d];
+  assert {:msg "Action at 20.3 ('readoff') for actor instance 'adj' might not preserve the channel invariant (#117)"} R[Net#c] == C[Net#e];
+  assert {:msg "Action at 20.3 ('readoff') for actor instance 'adj' might not preserve the channel invariant (#118)"} (forall idx$: int :: 
+    (0 <= idx$) && (idx$ < C[Net#b]) ==> (M[Net#b][idx$] == M[Net#a][idx$])
+  );
+  assert {:msg "Action at 20.3 ('readoff') for actor instance 'adj' might not preserve the channel invariant (#119)"} (forall idx$: int :: 
+    (0 <= idx$) && (idx$ < C[Net#c]) ==> (M[Net#c][idx$] == M[Net#a][idx$])
+  );
+  assert {:msg "Action at 20.3 ('readoff') for actor instance 'adj' might not preserve the channel invariant (#120)"} (forall idx$: int :: 
+    (0 <= idx$) && (idx$ < C[Net#d]) ==> (M[Net#d][idx$] == M[Net#b][idx$])
+  );
+  assert {:msg "Action at 20.3 ('readoff') for actor instance 'adj' might not preserve the channel invariant (#121)"} (forall idx$: int :: 
+    (0 <= idx$) && (idx$ < C[Net#e]) ==> (M[Net#e][idx$] == M[Net#c][idx$])
+  );
+  assert {:msg "Action at 20.3 ('readoff') for actor instance 'adj' might not preserve the channel invariant (#122)"} (forall idx$: int :: 
+    (0 <= idx$) && (idx$ < C[Net#a]) ==> (SqnCh[Net#a][idx$] == idx$)
+  );
 }
-procedure Net#anon$3#Adjudicator#normal#12()
-  modifies C, R, M, St, SqnCh, SqnAct;
+procedure Net##Adjudicator#normal#12()
+  modifies C, R, M, I, St, SqnCh, SqnAct;
 {
   var St#next: State;
   var x1#i: int;
   var x2#j: int;
   var c_in#c: int;
-  assume L[Net#a] == (1 * Base#L);
-  assume 0 <= R[Net#a];
-  assume 0 <= C[Net#a];
-  assume (R[Net#a] + C[Net#a]) <= L[Net#a];
-  assume 0 <= R[Net#b];
-  assume 0 <= C[Net#b];
-  assume 0 <= R[Net#c];
-  assume 0 <= C[Net#c];
-  assume 0 <= R[Net#d];
-  assume 0 <= C[Net#d];
-  assume 0 <= R[Net#e];
-  assume 0 <= C[Net#e];
-  assume 0 <= R[Net#f];
-  assume 0 <= C[Net#f];
-  assume 0 <= R[Net#g];
-  assume 0 <= C[Net#g];
-  assume R[Net#g] == 0;
-  assume R[Net#a] == (R[Net#b] + C[Net#b]);
-  assume R[Net#a] == (R[Net#c] + C[Net#c]);
-  assume R[Net#b] == (R[Net#d] + C[Net#d]);
-  assume R[Net#c] == (R[Net#e] + C[Net#e]);
-  assume (forall idx$: int :: 
-    (0 <= idx$) && (idx$ < (R[Net#b] + C[Net#b])) ==> (M[Net#b][idx$] == M[Net#a][idx$])
-  );
-  assume (forall idx$: int :: 
-    (0 <= idx$) && (idx$ < (R[Net#c] + C[Net#c])) ==> (M[Net#c][idx$] == M[Net#a][idx$])
-  );
-  assume (forall idx$: int :: 
-    (0 <= idx$) && (idx$ < (R[Net#d] + C[Net#d])) ==> (M[Net#d][idx$] == M[Net#b][idx$])
-  );
-  assume (forall idx$: int :: 
-    (0 <= idx$) && (idx$ < (R[Net#e] + C[Net#e])) ==> (M[Net#e][idx$] == M[Net#c][idx$])
-  );
-  assume (forall idx$: int :: 
-    (0 <= idx$) && (idx$ < (R[Net#a] + C[Net#a])) ==> (SqnCh[Net#a][idx$] == idx$)
-  );
+  assume 0 <= I[Net#a];
+  assume I[Net#a] <= R[Net#a];
+  assume R[Net#a] <= C[Net#a];
+  assume 0 <= I[Net#b];
+  assume I[Net#b] <= R[Net#b];
+  assume R[Net#b] <= C[Net#b];
+  assume 0 <= I[Net#c];
+  assume I[Net#c] <= R[Net#c];
+  assume R[Net#c] <= C[Net#c];
+  assume 0 <= I[Net#d];
+  assume I[Net#d] <= R[Net#d];
+  assume R[Net#d] <= C[Net#d];
+  assume 0 <= I[Net#e];
+  assume I[Net#e] <= R[Net#e];
+  assume R[Net#e] <= C[Net#e];
+  assume 0 <= I[Net#f];
+  assume I[Net#f] <= R[Net#f];
+  assume R[Net#f] <= C[Net#f];
+  assume 0 <= I[Net#g];
+  assume I[Net#g] <= R[Net#g];
+  assume R[Net#g] <= C[Net#g];
+  assume I[Net#g] == R[Net#g];
   assume SqnAct[Net#spl] == R[Net#a];
   assume SqnAct[Net#pri] == R[Net#b];
   assume SqnAct[Net#sec] == R[Net#c];
   assume SqnAct[Net#adj] == R[Net#e];
   assume (forall i: int :: 
-    (0 <= i) && (i < (R[Net#a] + C[Net#a])) ==> (SqnCh[Net#a][i] == i)
+    (0 <= i) && (i < C[Net#a]) ==> (SqnCh[Net#a][i] == i)
   );
   assume (forall i: int :: 
-    (0 <= i) && (i < (R[Net#b] + C[Net#b])) ==> (SqnCh[Net#b][i] == i)
+    (0 <= i) && (i < C[Net#b]) ==> (SqnCh[Net#b][i] == i)
   );
   assume (forall i: int :: 
-    (0 <= i) && (i < (R[Net#c] + C[Net#c])) ==> (SqnCh[Net#c][i] == i)
+    (0 <= i) && (i < C[Net#c]) ==> (SqnCh[Net#c][i] == i)
   );
   assume (forall i: int :: 
-    (0 <= i) && (i < (R[Net#d] + C[Net#d])) ==> (SqnCh[Net#d][i] == i)
+    (0 <= i) && (i < C[Net#d]) ==> (SqnCh[Net#d][i] == i)
   );
   assume (forall i: int :: 
-    (0 <= i) && (i < (R[Net#e] + C[Net#e])) ==> (SqnCh[Net#e][i] == i)
+    (0 <= i) && (i < C[Net#e]) ==> (SqnCh[Net#e][i] == i)
   );
   assume (forall i: int :: 
-    (0 <= i) && (i < (R[Net#g] + C[Net#g])) ==> (SqnCh[Net#g][i] == i)
+    (0 <= i) && (i < C[Net#g]) ==> (SqnCh[Net#g][i] == i)
   );
-  assume C[Net#f] == 1;
-  assume (R[Net#g] + C[Net#g]) == R[Net#e];
+  assume (C[Net#f] - R[Net#f]) == 1;
+  assume C[Net#g] == R[Net#e];
   assume R[Net#e] == M[Net#f][R[Net#f]];
   assume (forall i: int :: 
-    (0 <= i) && (i < (R[Net#g] + C[Net#g])) ==> (SqnCh[Net#g][i] == i)
+    (0 <= i) && (i < C[Net#g]) ==> (SqnCh[Net#g][i] == i)
   );
-  if ((0 < R[Net#d]) && (0 < R[Net#e])) {
-    assume M[Net#d][R[Net#d] - 1] <= M[Net#e][R[Net#e] - 1];
-  }
   assume (forall i: int :: 
     (0 <= i) && (i < R[Net#e]) ==> (M[Net#g][i] == M[Net#e][i])
+  );
+  assume R[Net#a] == C[Net#b];
+  assume R[Net#a] == C[Net#c];
+  assume R[Net#b] == C[Net#d];
+  assume R[Net#c] == C[Net#e];
+  assume (forall idx$: int :: 
+    (0 <= idx$) && (idx$ < C[Net#b]) ==> (M[Net#b][idx$] == M[Net#a][idx$])
+  );
+  assume (forall idx$: int :: 
+    (0 <= idx$) && (idx$ < C[Net#c]) ==> (M[Net#c][idx$] == M[Net#a][idx$])
+  );
+  assume (forall idx$: int :: 
+    (0 <= idx$) && (idx$ < C[Net#d]) ==> (M[Net#d][idx$] == M[Net#b][idx$])
+  );
+  assume (forall idx$: int :: 
+    (0 <= idx$) && (idx$ < C[Net#e]) ==> (M[Net#e][idx$] == M[Net#c][idx$])
+  );
+  assume (forall idx$: int :: 
+    (0 <= idx$) && (idx$ < C[Net#a]) ==> (SqnCh[Net#a][idx$] == idx$)
   );
   assume (SqnCh[Net#d][R[Net#d] - 0] == SqnCh[Net#e][R[Net#e] - 0]) && (SqnCh[Net#d][R[Net#d] - 0] == M[Net#f][R[Net#f] - 0]);
   assume true;
-  assume (!((1 <= C[Net#d]) && (1 <= C[Net#f]) && (SqnCh[Net#d][R[Net#d] - 0] < M[Net#f][R[Net#f] - 0]))) && (1 <= C[Net#d]) && (1 <= C[Net#e]) && (1 <= C[Net#f]) && (SqnCh[Net#d][R[Net#d] - 0] == SqnCh[Net#e][R[Net#e] - 0]) && (SqnCh[Net#d][R[Net#d] - 0] == M[Net#f][R[Net#f] - 0]);
+  assume (!((1 <= (C[Net#d] - R[Net#d])) && (1 <= (C[Net#f] - R[Net#f])) && (SqnCh[Net#d][R[Net#d] - 0] < M[Net#f][R[Net#f] - 0]))) && (1 <= (C[Net#d] - R[Net#d])) && (1 <= (C[Net#e] - R[Net#e])) && (1 <= (C[Net#f] - R[Net#f])) && (SqnCh[Net#d][R[Net#d] - 0] == SqnCh[Net#e][R[Net#e] - 0]) && (SqnCh[Net#d][R[Net#d] - 0] == M[Net#f][R[Net#f] - 0]);
   x1#i := M[Net#d][R[Net#d]];
   R[Net#d] := R[Net#d] + 1;
-  C[Net#d] := C[Net#d] - 1;
   x2#j := M[Net#e][R[Net#e]];
   R[Net#e] := R[Net#e] + 1;
-  C[Net#e] := C[Net#e] - 1;
   c_in#c := M[Net#f][R[Net#f]];
   R[Net#f] := R[Net#f] + 1;
-  C[Net#f] := C[Net#f] - 1;
-  M[Net#g][R[Net#g] + C[Net#g]] := x1#i;
-  SqnCh[Net#g][R[Net#g] + C[Net#g]] := SqnAct[Net#adj];
+  M[Net#g][C[Net#g]] := x1#i;
+  SqnCh[Net#g][C[Net#g]] := SqnAct[Net#adj];
   C[Net#g] := C[Net#g] + 1;
-  M[Net#f][R[Net#f] + C[Net#f]] := c_in#c + 1;
-  SqnCh[Net#f][R[Net#f] + C[Net#f]] := SqnAct[Net#adj];
+  M[Net#f][C[Net#f]] := c_in#c + 1;
+  SqnCh[Net#f][C[Net#f]] := SqnAct[Net#adj];
   C[Net#f] := C[Net#f] + 1;
   SqnAct[Net#adj] := SqnAct[Net#adj] + 1;
-  assert {:msg "  Action at 14.3 ('normal') for actor instance 'adj' might not preserve the channel invariant (#125)"} R[Net#a] == (R[Net#b] + C[Net#b]);
-  assert {:msg "  Action at 14.3 ('normal') for actor instance 'adj' might not preserve the channel invariant (#126)"} R[Net#a] == (R[Net#c] + C[Net#c]);
-  assert {:msg "  Action at 14.3 ('normal') for actor instance 'adj' might not preserve the channel invariant (#127)"} R[Net#b] == (R[Net#d] + C[Net#d]);
-  assert {:msg "  Action at 14.3 ('normal') for actor instance 'adj' might not preserve the channel invariant (#128)"} R[Net#c] == (R[Net#e] + C[Net#e]);
-  assert {:msg "  Action at 14.3 ('normal') for actor instance 'adj' might not preserve the channel invariant (#129)"} (forall idx$: int :: 
-    (0 <= idx$) && (idx$ < (R[Net#b] + C[Net#b])) ==> (M[Net#b][idx$] == M[Net#a][idx$])
+  assert {:msg "41.15: Action at 14.3 ('normal') for actor instance 'adj' might not preserve the channel invariant (#123)"} SqnAct[Net#spl] == R[Net#a];
+  assert {:msg "42.15: Action at 14.3 ('normal') for actor instance 'adj' might not preserve the channel invariant (#124)"} SqnAct[Net#pri] == R[Net#b];
+  assert {:msg "43.15: Action at 14.3 ('normal') for actor instance 'adj' might not preserve the channel invariant (#125)"} SqnAct[Net#sec] == R[Net#c];
+  assert {:msg "44.15: Action at 14.3 ('normal') for actor instance 'adj' might not preserve the channel invariant (#126)"} SqnAct[Net#adj] == R[Net#e];
+  assert {:msg "46.16: Action at 14.3 ('normal') for actor instance 'adj' might not preserve the channel invariant (#127)"} (forall i: int :: 
+    (0 <= i) && (i < C[Net#a]) ==> (SqnCh[Net#a][i] == i)
   );
-  assert {:msg "  Action at 14.3 ('normal') for actor instance 'adj' might not preserve the channel invariant (#130)"} (forall idx$: int :: 
-    (0 <= idx$) && (idx$ < (R[Net#c] + C[Net#c])) ==> (M[Net#c][idx$] == M[Net#a][idx$])
+  assert {:msg "47.16: Action at 14.3 ('normal') for actor instance 'adj' might not preserve the channel invariant (#128)"} (forall i: int :: 
+    (0 <= i) && (i < C[Net#b]) ==> (SqnCh[Net#b][i] == i)
   );
-  assert {:msg "  Action at 14.3 ('normal') for actor instance 'adj' might not preserve the channel invariant (#131)"} (forall idx$: int :: 
-    (0 <= idx$) && (idx$ < (R[Net#d] + C[Net#d])) ==> (M[Net#d][idx$] == M[Net#b][idx$])
+  assert {:msg "48.16: Action at 14.3 ('normal') for actor instance 'adj' might not preserve the channel invariant (#129)"} (forall i: int :: 
+    (0 <= i) && (i < C[Net#c]) ==> (SqnCh[Net#c][i] == i)
   );
-  assert {:msg "  Action at 14.3 ('normal') for actor instance 'adj' might not preserve the channel invariant (#132)"} (forall idx$: int :: 
-    (0 <= idx$) && (idx$ < (R[Net#e] + C[Net#e])) ==> (M[Net#e][idx$] == M[Net#c][idx$])
+  assert {:msg "49.16: Action at 14.3 ('normal') for actor instance 'adj' might not preserve the channel invariant (#130)"} (forall i: int :: 
+    (0 <= i) && (i < C[Net#d]) ==> (SqnCh[Net#d][i] == i)
   );
-  assert {:msg "  Action at 14.3 ('normal') for actor instance 'adj' might not preserve the channel invariant (#133)"} (forall idx$: int :: 
-    (0 <= idx$) && (idx$ < (R[Net#a] + C[Net#a])) ==> (SqnCh[Net#a][idx$] == idx$)
+  assert {:msg "50.16: Action at 14.3 ('normal') for actor instance 'adj' might not preserve the channel invariant (#131)"} (forall i: int :: 
+    (0 <= i) && (i < C[Net#e]) ==> (SqnCh[Net#e][i] == i)
   );
-  assert {:msg "  40.15: Action at 14.3 ('normal') for actor instance 'adj' might not preserve the channel invariant (#134)"} SqnAct[Net#spl] == R[Net#a];
-  assert {:msg "  41.15: Action at 14.3 ('normal') for actor instance 'adj' might not preserve the channel invariant (#135)"} SqnAct[Net#pri] == R[Net#b];
-  assert {:msg "  42.15: Action at 14.3 ('normal') for actor instance 'adj' might not preserve the channel invariant (#136)"} SqnAct[Net#sec] == R[Net#c];
-  assert {:msg "  43.15: Action at 14.3 ('normal') for actor instance 'adj' might not preserve the channel invariant (#137)"} SqnAct[Net#adj] == R[Net#e];
-  assert {:msg "  45.16: Action at 14.3 ('normal') for actor instance 'adj' might not preserve the channel invariant (#138)"} (forall i: int :: 
-    (0 <= i) && (i < (R[Net#a] + C[Net#a])) ==> (SqnCh[Net#a][i] == i)
+  assert {:msg "51.16: Action at 14.3 ('normal') for actor instance 'adj' might not preserve the channel invariant (#132)"} (forall i: int :: 
+    (0 <= i) && (i < C[Net#g]) ==> (SqnCh[Net#g][i] == i)
   );
-  assert {:msg "  46.16: Action at 14.3 ('normal') for actor instance 'adj' might not preserve the channel invariant (#139)"} (forall i: int :: 
-    (0 <= i) && (i < (R[Net#b] + C[Net#b])) ==> (SqnCh[Net#b][i] == i)
+  assert {:msg "53.15: Action at 14.3 ('normal') for actor instance 'adj' might not preserve the channel invariant (#133)"} (C[Net#f] - R[Net#f]) == 1;
+  assert {:msg "54.15: Action at 14.3 ('normal') for actor instance 'adj' might not preserve the channel invariant (#134)"} C[Net#g] == R[Net#e];
+  assert {:msg "55.15: Action at 14.3 ('normal') for actor instance 'adj' might not preserve the channel invariant (#135)"} R[Net#e] == M[Net#f][R[Net#f]];
+  assert {:msg "56.16: Action at 14.3 ('normal') for actor instance 'adj' might not preserve the channel invariant (#136)"} (forall i: int :: 
+    (0 <= i) && (i < C[Net#g]) ==> (SqnCh[Net#g][i] == i)
   );
-  assert {:msg "  47.16: Action at 14.3 ('normal') for actor instance 'adj' might not preserve the channel invariant (#140)"} (forall i: int :: 
-    (0 <= i) && (i < (R[Net#c] + C[Net#c])) ==> (SqnCh[Net#c][i] == i)
-  );
-  assert {:msg "  48.16: Action at 14.3 ('normal') for actor instance 'adj' might not preserve the channel invariant (#141)"} (forall i: int :: 
-    (0 <= i) && (i < (R[Net#d] + C[Net#d])) ==> (SqnCh[Net#d][i] == i)
-  );
-  assert {:msg "  49.16: Action at 14.3 ('normal') for actor instance 'adj' might not preserve the channel invariant (#142)"} (forall i: int :: 
-    (0 <= i) && (i < (R[Net#e] + C[Net#e])) ==> (SqnCh[Net#e][i] == i)
-  );
-  assert {:msg "  50.16: Action at 14.3 ('normal') for actor instance 'adj' might not preserve the channel invariant (#143)"} (forall i: int :: 
-    (0 <= i) && (i < (R[Net#g] + C[Net#g])) ==> (SqnCh[Net#g][i] == i)
-  );
-  assert {:msg "  52.15: Action at 14.3 ('normal') for actor instance 'adj' might not preserve the channel invariant (#144)"} C[Net#f] == 1;
-  assert {:msg "  53.15: Action at 14.3 ('normal') for actor instance 'adj' might not preserve the channel invariant (#145)"} (R[Net#g] + C[Net#g]) == R[Net#e];
-  assert {:msg "  54.15: Action at 14.3 ('normal') for actor instance 'adj' might not preserve the channel invariant (#146)"} R[Net#e] == M[Net#f][R[Net#f]];
-  assert {:msg "  55.16: Action at 14.3 ('normal') for actor instance 'adj' might not preserve the channel invariant (#147)"} (forall i: int :: 
-    (0 <= i) && (i < (R[Net#g] + C[Net#g])) ==> (SqnCh[Net#g][i] == i)
-  );
-  if ((0 < R[Net#d]) && (0 < R[Net#e])) {
-    assert {:msg "  57.42: Action at 14.3 ('normal') for actor instance 'adj' might not preserve the channel invariant (#148)"} M[Net#d][R[Net#d] - 1] <= M[Net#e][R[Net#e] - 1];
-  }
-  assert {:msg "  58.16: Action at 14.3 ('normal') for actor instance 'adj' might not preserve the channel invariant (#149)"} (forall i: int :: 
+  assert {:msg "59.16: Action at 14.3 ('normal') for actor instance 'adj' might not preserve the channel invariant (#137)"} (forall i: int :: 
     (0 <= i) && (i < R[Net#e]) ==> (M[Net#g][i] == M[Net#e][i])
   );
+  assert {:msg "Action at 14.3 ('normal') for actor instance 'adj' might not preserve the channel invariant (#138)"} R[Net#a] == C[Net#b];
+  assert {:msg "Action at 14.3 ('normal') for actor instance 'adj' might not preserve the channel invariant (#139)"} R[Net#a] == C[Net#c];
+  assert {:msg "Action at 14.3 ('normal') for actor instance 'adj' might not preserve the channel invariant (#140)"} R[Net#b] == C[Net#d];
+  assert {:msg "Action at 14.3 ('normal') for actor instance 'adj' might not preserve the channel invariant (#141)"} R[Net#c] == C[Net#e];
+  assert {:msg "Action at 14.3 ('normal') for actor instance 'adj' might not preserve the channel invariant (#142)"} (forall idx$: int :: 
+    (0 <= idx$) && (idx$ < C[Net#b]) ==> (M[Net#b][idx$] == M[Net#a][idx$])
+  );
+  assert {:msg "Action at 14.3 ('normal') for actor instance 'adj' might not preserve the channel invariant (#143)"} (forall idx$: int :: 
+    (0 <= idx$) && (idx$ < C[Net#c]) ==> (M[Net#c][idx$] == M[Net#a][idx$])
+  );
+  assert {:msg "Action at 14.3 ('normal') for actor instance 'adj' might not preserve the channel invariant (#144)"} (forall idx$: int :: 
+    (0 <= idx$) && (idx$ < C[Net#d]) ==> (M[Net#d][idx$] == M[Net#b][idx$])
+  );
+  assert {:msg "Action at 14.3 ('normal') for actor instance 'adj' might not preserve the channel invariant (#145)"} (forall idx$: int :: 
+    (0 <= idx$) && (idx$ < C[Net#e]) ==> (M[Net#e][idx$] == M[Net#c][idx$])
+  );
+  assert {:msg "Action at 14.3 ('normal') for actor instance 'adj' might not preserve the channel invariant (#146)"} (forall idx$: int :: 
+    (0 <= idx$) && (idx$ < C[Net#a]) ==> (SqnCh[Net#a][idx$] == idx$)
+  );
 }
-procedure Net#anon$3#Adjudicator#timeout#13()
-  modifies C, R, M, St, SqnCh, SqnAct;
+procedure Net##Adjudicator#timeout#13()
+  modifies C, R, M, I, St, SqnCh, SqnAct;
 {
   var St#next: State;
   var x2#j: int;
   var c_in#c: int;
-  assume L[Net#a] == (1 * Base#L);
-  assume 0 <= R[Net#a];
-  assume 0 <= C[Net#a];
-  assume (R[Net#a] + C[Net#a]) <= L[Net#a];
-  assume 0 <= R[Net#b];
-  assume 0 <= C[Net#b];
-  assume 0 <= R[Net#c];
-  assume 0 <= C[Net#c];
-  assume 0 <= R[Net#d];
-  assume 0 <= C[Net#d];
-  assume 0 <= R[Net#e];
-  assume 0 <= C[Net#e];
-  assume 0 <= R[Net#f];
-  assume 0 <= C[Net#f];
-  assume 0 <= R[Net#g];
-  assume 0 <= C[Net#g];
-  assume R[Net#g] == 0;
-  assume R[Net#a] == (R[Net#b] + C[Net#b]);
-  assume R[Net#a] == (R[Net#c] + C[Net#c]);
-  assume R[Net#b] == (R[Net#d] + C[Net#d]);
-  assume R[Net#c] == (R[Net#e] + C[Net#e]);
-  assume (forall idx$: int :: 
-    (0 <= idx$) && (idx$ < (R[Net#b] + C[Net#b])) ==> (M[Net#b][idx$] == M[Net#a][idx$])
-  );
-  assume (forall idx$: int :: 
-    (0 <= idx$) && (idx$ < (R[Net#c] + C[Net#c])) ==> (M[Net#c][idx$] == M[Net#a][idx$])
-  );
-  assume (forall idx$: int :: 
-    (0 <= idx$) && (idx$ < (R[Net#d] + C[Net#d])) ==> (M[Net#d][idx$] == M[Net#b][idx$])
-  );
-  assume (forall idx$: int :: 
-    (0 <= idx$) && (idx$ < (R[Net#e] + C[Net#e])) ==> (M[Net#e][idx$] == M[Net#c][idx$])
-  );
-  assume (forall idx$: int :: 
-    (0 <= idx$) && (idx$ < (R[Net#a] + C[Net#a])) ==> (SqnCh[Net#a][idx$] == idx$)
-  );
+  assume 0 <= I[Net#a];
+  assume I[Net#a] <= R[Net#a];
+  assume R[Net#a] <= C[Net#a];
+  assume 0 <= I[Net#b];
+  assume I[Net#b] <= R[Net#b];
+  assume R[Net#b] <= C[Net#b];
+  assume 0 <= I[Net#c];
+  assume I[Net#c] <= R[Net#c];
+  assume R[Net#c] <= C[Net#c];
+  assume 0 <= I[Net#d];
+  assume I[Net#d] <= R[Net#d];
+  assume R[Net#d] <= C[Net#d];
+  assume 0 <= I[Net#e];
+  assume I[Net#e] <= R[Net#e];
+  assume R[Net#e] <= C[Net#e];
+  assume 0 <= I[Net#f];
+  assume I[Net#f] <= R[Net#f];
+  assume R[Net#f] <= C[Net#f];
+  assume 0 <= I[Net#g];
+  assume I[Net#g] <= R[Net#g];
+  assume R[Net#g] <= C[Net#g];
+  assume I[Net#g] == R[Net#g];
   assume SqnAct[Net#spl] == R[Net#a];
   assume SqnAct[Net#pri] == R[Net#b];
   assume SqnAct[Net#sec] == R[Net#c];
   assume SqnAct[Net#adj] == R[Net#e];
   assume (forall i: int :: 
-    (0 <= i) && (i < (R[Net#a] + C[Net#a])) ==> (SqnCh[Net#a][i] == i)
+    (0 <= i) && (i < C[Net#a]) ==> (SqnCh[Net#a][i] == i)
   );
   assume (forall i: int :: 
-    (0 <= i) && (i < (R[Net#b] + C[Net#b])) ==> (SqnCh[Net#b][i] == i)
+    (0 <= i) && (i < C[Net#b]) ==> (SqnCh[Net#b][i] == i)
   );
   assume (forall i: int :: 
-    (0 <= i) && (i < (R[Net#c] + C[Net#c])) ==> (SqnCh[Net#c][i] == i)
+    (0 <= i) && (i < C[Net#c]) ==> (SqnCh[Net#c][i] == i)
   );
   assume (forall i: int :: 
-    (0 <= i) && (i < (R[Net#d] + C[Net#d])) ==> (SqnCh[Net#d][i] == i)
+    (0 <= i) && (i < C[Net#d]) ==> (SqnCh[Net#d][i] == i)
   );
   assume (forall i: int :: 
-    (0 <= i) && (i < (R[Net#e] + C[Net#e])) ==> (SqnCh[Net#e][i] == i)
+    (0 <= i) && (i < C[Net#e]) ==> (SqnCh[Net#e][i] == i)
   );
   assume (forall i: int :: 
-    (0 <= i) && (i < (R[Net#g] + C[Net#g])) ==> (SqnCh[Net#g][i] == i)
+    (0 <= i) && (i < C[Net#g]) ==> (SqnCh[Net#g][i] == i)
   );
-  assume C[Net#f] == 1;
-  assume (R[Net#g] + C[Net#g]) == R[Net#e];
+  assume (C[Net#f] - R[Net#f]) == 1;
+  assume C[Net#g] == R[Net#e];
   assume R[Net#e] == M[Net#f][R[Net#f]];
   assume (forall i: int :: 
-    (0 <= i) && (i < (R[Net#g] + C[Net#g])) ==> (SqnCh[Net#g][i] == i)
+    (0 <= i) && (i < C[Net#g]) ==> (SqnCh[Net#g][i] == i)
   );
-  if ((0 < R[Net#d]) && (0 < R[Net#e])) {
-    assume M[Net#d][R[Net#d] - 1] <= M[Net#e][R[Net#e] - 1];
-  }
   assume (forall i: int :: 
     (0 <= i) && (i < R[Net#e]) ==> (M[Net#g][i] == M[Net#e][i])
+  );
+  assume R[Net#a] == C[Net#b];
+  assume R[Net#a] == C[Net#c];
+  assume R[Net#b] == C[Net#d];
+  assume R[Net#c] == C[Net#e];
+  assume (forall idx$: int :: 
+    (0 <= idx$) && (idx$ < C[Net#b]) ==> (M[Net#b][idx$] == M[Net#a][idx$])
+  );
+  assume (forall idx$: int :: 
+    (0 <= idx$) && (idx$ < C[Net#c]) ==> (M[Net#c][idx$] == M[Net#a][idx$])
+  );
+  assume (forall idx$: int :: 
+    (0 <= idx$) && (idx$ < C[Net#d]) ==> (M[Net#d][idx$] == M[Net#b][idx$])
+  );
+  assume (forall idx$: int :: 
+    (0 <= idx$) && (idx$ < C[Net#e]) ==> (M[Net#e][idx$] == M[Net#c][idx$])
+  );
+  assume (forall idx$: int :: 
+    (0 <= idx$) && (idx$ < C[Net#a]) ==> (SqnCh[Net#a][idx$] == idx$)
   );
   assume true;
-  assume (!((1 <= C[Net#d]) && (1 <= C[Net#f]) && (SqnCh[Net#d][R[Net#d] - 0] < M[Net#f][R[Net#f] - 0]))) && (!((1 <= C[Net#d]) && (1 <= C[Net#e]) && (1 <= C[Net#f]) && (SqnCh[Net#d][R[Net#d] - 0] == SqnCh[Net#e][R[Net#e] - 0]) && (SqnCh[Net#d][R[Net#d] - 0] == M[Net#f][R[Net#f] - 0]))) && (1 <= C[Net#e]) && (1 <= C[Net#f]);
+  assume (!((1 <= (C[Net#d] - R[Net#d])) && (1 <= (C[Net#f] - R[Net#f])) && (SqnCh[Net#d][R[Net#d] - 0] < M[Net#f][R[Net#f] - 0]))) && (!((1 <= (C[Net#d] - R[Net#d])) && (1 <= (C[Net#e] - R[Net#e])) && (1 <= (C[Net#f] - R[Net#f])) && (SqnCh[Net#d][R[Net#d] - 0] == SqnCh[Net#e][R[Net#e] - 0]) && (SqnCh[Net#d][R[Net#d] - 0] == M[Net#f][R[Net#f] - 0]))) && (1 <= (C[Net#e] - R[Net#e])) && (1 <= (C[Net#f] - R[Net#f]));
   x2#j := M[Net#e][R[Net#e]];
   R[Net#e] := R[Net#e] + 1;
-  C[Net#e] := C[Net#e] - 1;
   c_in#c := M[Net#f][R[Net#f]];
   R[Net#f] := R[Net#f] + 1;
-  C[Net#f] := C[Net#f] - 1;
-  M[Net#g][R[Net#g] + C[Net#g]] := x2#j;
-  SqnCh[Net#g][R[Net#g] + C[Net#g]] := SqnAct[Net#adj];
+  M[Net#g][C[Net#g]] := x2#j;
+  SqnCh[Net#g][C[Net#g]] := SqnAct[Net#adj];
   C[Net#g] := C[Net#g] + 1;
-  M[Net#f][R[Net#f] + C[Net#f]] := c_in#c + 1;
-  SqnCh[Net#f][R[Net#f] + C[Net#f]] := SqnAct[Net#adj];
+  M[Net#f][C[Net#f]] := c_in#c + 1;
+  SqnCh[Net#f][C[Net#f]] := SqnAct[Net#adj];
   C[Net#f] := C[Net#f] + 1;
   SqnAct[Net#adj] := SqnAct[Net#adj] + 1;
-  assert {:msg "  Action at 18.3 ('timeout') for actor instance 'adj' might not preserve the channel invariant (#150)"} R[Net#a] == (R[Net#b] + C[Net#b]);
-  assert {:msg "  Action at 18.3 ('timeout') for actor instance 'adj' might not preserve the channel invariant (#151)"} R[Net#a] == (R[Net#c] + C[Net#c]);
-  assert {:msg "  Action at 18.3 ('timeout') for actor instance 'adj' might not preserve the channel invariant (#152)"} R[Net#b] == (R[Net#d] + C[Net#d]);
-  assert {:msg "  Action at 18.3 ('timeout') for actor instance 'adj' might not preserve the channel invariant (#153)"} R[Net#c] == (R[Net#e] + C[Net#e]);
-  assert {:msg "  Action at 18.3 ('timeout') for actor instance 'adj' might not preserve the channel invariant (#154)"} (forall idx$: int :: 
-    (0 <= idx$) && (idx$ < (R[Net#b] + C[Net#b])) ==> (M[Net#b][idx$] == M[Net#a][idx$])
+  assert {:msg "41.15: Action at 18.3 ('timeout') for actor instance 'adj' might not preserve the channel invariant (#147)"} SqnAct[Net#spl] == R[Net#a];
+  assert {:msg "42.15: Action at 18.3 ('timeout') for actor instance 'adj' might not preserve the channel invariant (#148)"} SqnAct[Net#pri] == R[Net#b];
+  assert {:msg "43.15: Action at 18.3 ('timeout') for actor instance 'adj' might not preserve the channel invariant (#149)"} SqnAct[Net#sec] == R[Net#c];
+  assert {:msg "44.15: Action at 18.3 ('timeout') for actor instance 'adj' might not preserve the channel invariant (#150)"} SqnAct[Net#adj] == R[Net#e];
+  assert {:msg "46.16: Action at 18.3 ('timeout') for actor instance 'adj' might not preserve the channel invariant (#151)"} (forall i: int :: 
+    (0 <= i) && (i < C[Net#a]) ==> (SqnCh[Net#a][i] == i)
   );
-  assert {:msg "  Action at 18.3 ('timeout') for actor instance 'adj' might not preserve the channel invariant (#155)"} (forall idx$: int :: 
-    (0 <= idx$) && (idx$ < (R[Net#c] + C[Net#c])) ==> (M[Net#c][idx$] == M[Net#a][idx$])
+  assert {:msg "47.16: Action at 18.3 ('timeout') for actor instance 'adj' might not preserve the channel invariant (#152)"} (forall i: int :: 
+    (0 <= i) && (i < C[Net#b]) ==> (SqnCh[Net#b][i] == i)
   );
-  assert {:msg "  Action at 18.3 ('timeout') for actor instance 'adj' might not preserve the channel invariant (#156)"} (forall idx$: int :: 
-    (0 <= idx$) && (idx$ < (R[Net#d] + C[Net#d])) ==> (M[Net#d][idx$] == M[Net#b][idx$])
+  assert {:msg "48.16: Action at 18.3 ('timeout') for actor instance 'adj' might not preserve the channel invariant (#153)"} (forall i: int :: 
+    (0 <= i) && (i < C[Net#c]) ==> (SqnCh[Net#c][i] == i)
   );
-  assert {:msg "  Action at 18.3 ('timeout') for actor instance 'adj' might not preserve the channel invariant (#157)"} (forall idx$: int :: 
-    (0 <= idx$) && (idx$ < (R[Net#e] + C[Net#e])) ==> (M[Net#e][idx$] == M[Net#c][idx$])
+  assert {:msg "49.16: Action at 18.3 ('timeout') for actor instance 'adj' might not preserve the channel invariant (#154)"} (forall i: int :: 
+    (0 <= i) && (i < C[Net#d]) ==> (SqnCh[Net#d][i] == i)
   );
-  assert {:msg "  Action at 18.3 ('timeout') for actor instance 'adj' might not preserve the channel invariant (#158)"} (forall idx$: int :: 
-    (0 <= idx$) && (idx$ < (R[Net#a] + C[Net#a])) ==> (SqnCh[Net#a][idx$] == idx$)
+  assert {:msg "50.16: Action at 18.3 ('timeout') for actor instance 'adj' might not preserve the channel invariant (#155)"} (forall i: int :: 
+    (0 <= i) && (i < C[Net#e]) ==> (SqnCh[Net#e][i] == i)
   );
-  assert {:msg "  40.15: Action at 18.3 ('timeout') for actor instance 'adj' might not preserve the channel invariant (#159)"} SqnAct[Net#spl] == R[Net#a];
-  assert {:msg "  41.15: Action at 18.3 ('timeout') for actor instance 'adj' might not preserve the channel invariant (#160)"} SqnAct[Net#pri] == R[Net#b];
-  assert {:msg "  42.15: Action at 18.3 ('timeout') for actor instance 'adj' might not preserve the channel invariant (#161)"} SqnAct[Net#sec] == R[Net#c];
-  assert {:msg "  43.15: Action at 18.3 ('timeout') for actor instance 'adj' might not preserve the channel invariant (#162)"} SqnAct[Net#adj] == R[Net#e];
-  assert {:msg "  45.16: Action at 18.3 ('timeout') for actor instance 'adj' might not preserve the channel invariant (#163)"} (forall i: int :: 
-    (0 <= i) && (i < (R[Net#a] + C[Net#a])) ==> (SqnCh[Net#a][i] == i)
+  assert {:msg "51.16: Action at 18.3 ('timeout') for actor instance 'adj' might not preserve the channel invariant (#156)"} (forall i: int :: 
+    (0 <= i) && (i < C[Net#g]) ==> (SqnCh[Net#g][i] == i)
   );
-  assert {:msg "  46.16: Action at 18.3 ('timeout') for actor instance 'adj' might not preserve the channel invariant (#164)"} (forall i: int :: 
-    (0 <= i) && (i < (R[Net#b] + C[Net#b])) ==> (SqnCh[Net#b][i] == i)
+  assert {:msg "53.15: Action at 18.3 ('timeout') for actor instance 'adj' might not preserve the channel invariant (#157)"} (C[Net#f] - R[Net#f]) == 1;
+  assert {:msg "54.15: Action at 18.3 ('timeout') for actor instance 'adj' might not preserve the channel invariant (#158)"} C[Net#g] == R[Net#e];
+  assert {:msg "55.15: Action at 18.3 ('timeout') for actor instance 'adj' might not preserve the channel invariant (#159)"} R[Net#e] == M[Net#f][R[Net#f]];
+  assert {:msg "56.16: Action at 18.3 ('timeout') for actor instance 'adj' might not preserve the channel invariant (#160)"} (forall i: int :: 
+    (0 <= i) && (i < C[Net#g]) ==> (SqnCh[Net#g][i] == i)
   );
-  assert {:msg "  47.16: Action at 18.3 ('timeout') for actor instance 'adj' might not preserve the channel invariant (#165)"} (forall i: int :: 
-    (0 <= i) && (i < (R[Net#c] + C[Net#c])) ==> (SqnCh[Net#c][i] == i)
-  );
-  assert {:msg "  48.16: Action at 18.3 ('timeout') for actor instance 'adj' might not preserve the channel invariant (#166)"} (forall i: int :: 
-    (0 <= i) && (i < (R[Net#d] + C[Net#d])) ==> (SqnCh[Net#d][i] == i)
-  );
-  assert {:msg "  49.16: Action at 18.3 ('timeout') for actor instance 'adj' might not preserve the channel invariant (#167)"} (forall i: int :: 
-    (0 <= i) && (i < (R[Net#e] + C[Net#e])) ==> (SqnCh[Net#e][i] == i)
-  );
-  assert {:msg "  50.16: Action at 18.3 ('timeout') for actor instance 'adj' might not preserve the channel invariant (#168)"} (forall i: int :: 
-    (0 <= i) && (i < (R[Net#g] + C[Net#g])) ==> (SqnCh[Net#g][i] == i)
-  );
-  assert {:msg "  52.15: Action at 18.3 ('timeout') for actor instance 'adj' might not preserve the channel invariant (#169)"} C[Net#f] == 1;
-  assert {:msg "  53.15: Action at 18.3 ('timeout') for actor instance 'adj' might not preserve the channel invariant (#170)"} (R[Net#g] + C[Net#g]) == R[Net#e];
-  assert {:msg "  54.15: Action at 18.3 ('timeout') for actor instance 'adj' might not preserve the channel invariant (#171)"} R[Net#e] == M[Net#f][R[Net#f]];
-  assert {:msg "  55.16: Action at 18.3 ('timeout') for actor instance 'adj' might not preserve the channel invariant (#172)"} (forall i: int :: 
-    (0 <= i) && (i < (R[Net#g] + C[Net#g])) ==> (SqnCh[Net#g][i] == i)
-  );
-  if ((0 < R[Net#d]) && (0 < R[Net#e])) {
-    assert {:msg "  57.42: Action at 18.3 ('timeout') for actor instance 'adj' might not preserve the channel invariant (#173)"} M[Net#d][R[Net#d] - 1] <= M[Net#e][R[Net#e] - 1];
-  }
-  assert {:msg "  58.16: Action at 18.3 ('timeout') for actor instance 'adj' might not preserve the channel invariant (#174)"} (forall i: int :: 
+  assert {:msg "59.16: Action at 18.3 ('timeout') for actor instance 'adj' might not preserve the channel invariant (#161)"} (forall i: int :: 
     (0 <= i) && (i < R[Net#e]) ==> (M[Net#g][i] == M[Net#e][i])
   );
+  assert {:msg "Action at 18.3 ('timeout') for actor instance 'adj' might not preserve the channel invariant (#162)"} R[Net#a] == C[Net#b];
+  assert {:msg "Action at 18.3 ('timeout') for actor instance 'adj' might not preserve the channel invariant (#163)"} R[Net#a] == C[Net#c];
+  assert {:msg "Action at 18.3 ('timeout') for actor instance 'adj' might not preserve the channel invariant (#164)"} R[Net#b] == C[Net#d];
+  assert {:msg "Action at 18.3 ('timeout') for actor instance 'adj' might not preserve the channel invariant (#165)"} R[Net#c] == C[Net#e];
+  assert {:msg "Action at 18.3 ('timeout') for actor instance 'adj' might not preserve the channel invariant (#166)"} (forall idx$: int :: 
+    (0 <= idx$) && (idx$ < C[Net#b]) ==> (M[Net#b][idx$] == M[Net#a][idx$])
+  );
+  assert {:msg "Action at 18.3 ('timeout') for actor instance 'adj' might not preserve the channel invariant (#167)"} (forall idx$: int :: 
+    (0 <= idx$) && (idx$ < C[Net#c]) ==> (M[Net#c][idx$] == M[Net#a][idx$])
+  );
+  assert {:msg "Action at 18.3 ('timeout') for actor instance 'adj' might not preserve the channel invariant (#168)"} (forall idx$: int :: 
+    (0 <= idx$) && (idx$ < C[Net#d]) ==> (M[Net#d][idx$] == M[Net#b][idx$])
+  );
+  assert {:msg "Action at 18.3 ('timeout') for actor instance 'adj' might not preserve the channel invariant (#169)"} (forall idx$: int :: 
+    (0 <= idx$) && (idx$ < C[Net#e]) ==> (M[Net#e][idx$] == M[Net#c][idx$])
+  );
+  assert {:msg "Action at 18.3 ('timeout') for actor instance 'adj' might not preserve the channel invariant (#170)"} (forall idx$: int :: 
+    (0 <= idx$) && (idx$ < C[Net#a]) ==> (SqnCh[Net#a][idx$] == idx$)
+  );
 }
-procedure Net#anon$3#exit#14()
-  modifies C, R, M, St, SqnCh, SqnAct;
+procedure Net#anon$3#entry#14()
+  modifies C, R, M, I, St, SqnCh, SqnAct;
 {
-  assume L[Net#a] == (1 * Base#L);
-  assume 0 <= R[Net#a];
-  assume 0 <= C[Net#a];
-  assume (R[Net#a] + C[Net#a]) <= L[Net#a];
-  assume 0 <= R[Net#b];
-  assume 0 <= C[Net#b];
-  assume 0 <= R[Net#c];
-  assume 0 <= C[Net#c];
-  assume 0 <= R[Net#d];
-  assume 0 <= C[Net#d];
-  assume 0 <= R[Net#e];
-  assume 0 <= C[Net#e];
-  assume 0 <= R[Net#f];
-  assume 0 <= C[Net#f];
-  assume 0 <= R[Net#g];
-  assume 0 <= C[Net#g];
-  assume R[Net#g] == 0;
-  assume R[Net#a] == (R[Net#b] + C[Net#b]);
-  assume R[Net#a] == (R[Net#c] + C[Net#c]);
-  assume R[Net#b] == (R[Net#d] + C[Net#d]);
-  assume R[Net#c] == (R[Net#e] + C[Net#e]);
-  assume (forall idx$: int :: 
-    (0 <= idx$) && (idx$ < (R[Net#b] + C[Net#b])) ==> (M[Net#b][idx$] == M[Net#a][idx$])
-  );
-  assume (forall idx$: int :: 
-    (0 <= idx$) && (idx$ < (R[Net#c] + C[Net#c])) ==> (M[Net#c][idx$] == M[Net#a][idx$])
-  );
-  assume (forall idx$: int :: 
-    (0 <= idx$) && (idx$ < (R[Net#d] + C[Net#d])) ==> (M[Net#d][idx$] == M[Net#b][idx$])
-  );
-  assume (forall idx$: int :: 
-    (0 <= idx$) && (idx$ < (R[Net#e] + C[Net#e])) ==> (M[Net#e][idx$] == M[Net#c][idx$])
-  );
-  assume (forall idx$: int :: 
-    (0 <= idx$) && (idx$ < (R[Net#a] + C[Net#a])) ==> (SqnCh[Net#a][idx$] == idx$)
-  );
+  assume 0 <= I[Net#a];
+  assume I[Net#a] <= R[Net#a];
+  assume R[Net#a] <= C[Net#a];
+  assume 0 <= I[Net#b];
+  assume I[Net#b] <= R[Net#b];
+  assume R[Net#b] <= C[Net#b];
+  assume 0 <= I[Net#c];
+  assume I[Net#c] <= R[Net#c];
+  assume R[Net#c] <= C[Net#c];
+  assume 0 <= I[Net#d];
+  assume I[Net#d] <= R[Net#d];
+  assume R[Net#d] <= C[Net#d];
+  assume 0 <= I[Net#e];
+  assume I[Net#e] <= R[Net#e];
+  assume R[Net#e] <= C[Net#e];
+  assume 0 <= I[Net#f];
+  assume I[Net#f] <= R[Net#f];
+  assume R[Net#f] <= C[Net#f];
+  assume 0 <= I[Net#g];
+  assume I[Net#g] <= R[Net#g];
+  assume R[Net#g] <= C[Net#g];
+  assume I[Net#g] == R[Net#g];
+  assume I == R;
+  assume R[Net#a] == C[Net#a];
+  assume R[Net#b] == C[Net#b];
+  assume R[Net#c] == C[Net#c];
+  assume R[Net#d] == C[Net#d];
+  assume R[Net#e] == C[Net#e];
+  assume R[Net#f] == C[Net#f];
+  assume R[Net#g] == C[Net#g];
+  C[Net#f] := C[Net#f] + 1;
+  assume R[Net#e] == M[Net#f][R[Net#f]];
   assume SqnAct[Net#spl] == R[Net#a];
   assume SqnAct[Net#pri] == R[Net#b];
   assume SqnAct[Net#sec] == R[Net#c];
   assume SqnAct[Net#adj] == R[Net#e];
   assume (forall i: int :: 
-    (0 <= i) && (i < (R[Net#a] + C[Net#a])) ==> (SqnCh[Net#a][i] == i)
+    (0 <= i) && (i < C[Net#a]) ==> (SqnCh[Net#a][i] == i)
   );
   assume (forall i: int :: 
-    (0 <= i) && (i < (R[Net#b] + C[Net#b])) ==> (SqnCh[Net#b][i] == i)
+    (0 <= i) && (i < C[Net#b]) ==> (SqnCh[Net#b][i] == i)
   );
   assume (forall i: int :: 
-    (0 <= i) && (i < (R[Net#c] + C[Net#c])) ==> (SqnCh[Net#c][i] == i)
+    (0 <= i) && (i < C[Net#c]) ==> (SqnCh[Net#c][i] == i)
   );
   assume (forall i: int :: 
-    (0 <= i) && (i < (R[Net#d] + C[Net#d])) ==> (SqnCh[Net#d][i] == i)
+    (0 <= i) && (i < C[Net#d]) ==> (SqnCh[Net#d][i] == i)
   );
   assume (forall i: int :: 
-    (0 <= i) && (i < (R[Net#e] + C[Net#e])) ==> (SqnCh[Net#e][i] == i)
+    (0 <= i) && (i < C[Net#e]) ==> (SqnCh[Net#e][i] == i)
   );
   assume (forall i: int :: 
-    (0 <= i) && (i < (R[Net#g] + C[Net#g])) ==> (SqnCh[Net#g][i] == i)
+    (0 <= i) && (i < C[Net#g]) ==> (SqnCh[Net#g][i] == i)
   );
-  assume C[Net#f] == 1;
-  assume (R[Net#g] + C[Net#g]) == R[Net#e];
+  assume (C[Net#f] - R[Net#f]) == 1;
+  assume C[Net#g] == R[Net#e];
   assume R[Net#e] == M[Net#f][R[Net#f]];
   assume (forall i: int :: 
-    (0 <= i) && (i < (R[Net#g] + C[Net#g])) ==> (SqnCh[Net#g][i] == i)
+    (0 <= i) && (i < C[Net#g]) ==> (SqnCh[Net#g][i] == i)
   );
-  if ((0 < R[Net#d]) && (0 < R[Net#e])) {
-    assume M[Net#d][R[Net#d] - 1] <= M[Net#e][R[Net#e] - 1];
-  }
   assume (forall i: int :: 
     (0 <= i) && (i < R[Net#e]) ==> (M[Net#g][i] == M[Net#e][i])
   );
-  assume !((R[Net#a] + C[Net#a]) < L[Net#a]);
-  assume !(1 <= C[Net#a]);
-  assume !(1 <= C[Net#b]);
-  assume !(1 <= C[Net#c]);
-  assume !((!((1 <= C[Net#d]) && (1 <= C[Net#f]) && (SqnCh[Net#d][R[Net#d] - 0] < M[Net#f][R[Net#f] - 0]))) && (1 <= C[Net#d]) && (1 <= C[Net#e]) && (1 <= C[Net#f]) && (SqnCh[Net#d][R[Net#d] - 0] == SqnCh[Net#e][R[Net#e] - 0]) && (SqnCh[Net#d][R[Net#d] - 0] == M[Net#f][R[Net#f] - 0]));
-  assume !((!((1 <= C[Net#d]) && (1 <= C[Net#f]) && (SqnCh[Net#d][R[Net#d] - 0] < M[Net#f][R[Net#f] - 0]))) && (!((1 <= C[Net#d]) && (1 <= C[Net#e]) && (1 <= C[Net#f]) && (SqnCh[Net#d][R[Net#d] - 0] == SqnCh[Net#e][R[Net#e] - 0]) && (SqnCh[Net#d][R[Net#d] - 0] == M[Net#f][R[Net#f] - 0]))) && (1 <= C[Net#e]) && (1 <= C[Net#f]));
-  assume !((1 <= C[Net#d]) && (1 <= C[Net#f]) && (SqnCh[Net#d][R[Net#d] - 0] < M[Net#f][R[Net#f] - 0]));
-  assert {:msg "  33.14: Network action postcondition might not hold"} (forall i: int :: 
-    (0 <= i) && (i < (R[Net#g] + C[Net#g])) ==> (SqnCh[Net#g][i] == i)
+  assume R[Net#a] == C[Net#b];
+  assume R[Net#a] == C[Net#c];
+  assume R[Net#b] == C[Net#d];
+  assume R[Net#c] == C[Net#e];
+  assume (forall idx$: int :: 
+    (0 <= idx$) && (idx$ < C[Net#b]) ==> (M[Net#b][idx$] == M[Net#a][idx$])
   );
-  assert {:msg "  34.14: Network action postcondition might not hold"} (forall i: int :: 
-    (0 <= i) && (i < (R[Net#g] + C[Net#g])) ==> (M[Net#g][i] == M[Net#a][i])
+  assume (forall idx$: int :: 
+    (0 <= idx$) && (idx$ < C[Net#c]) ==> (M[Net#c][idx$] == M[Net#a][idx$])
   );
-  R[Net#g] := R[Net#g] + C[Net#g];
-  C[Net#g] := C[Net#g] - (1 * Base#L);
-  assert {:msg "  The network might not preserve the channel invariant"} R[Net#a] == (R[Net#b] + C[Net#b]);
-  assert {:msg "  The network might not preserve the channel invariant"} R[Net#a] == (R[Net#c] + C[Net#c]);
-  assert {:msg "  The network might not preserve the channel invariant"} R[Net#b] == (R[Net#d] + C[Net#d]);
-  assert {:msg "  The network might not preserve the channel invariant"} R[Net#c] == (R[Net#e] + C[Net#e]);
-  assert {:msg "  The network might not preserve the channel invariant"} (forall idx$: int :: 
-    (0 <= idx$) && (idx$ < (R[Net#b] + C[Net#b])) ==> (M[Net#b][idx$] == M[Net#a][idx$])
+  assume (forall idx$: int :: 
+    (0 <= idx$) && (idx$ < C[Net#d]) ==> (M[Net#d][idx$] == M[Net#b][idx$])
   );
-  assert {:msg "  The network might not preserve the channel invariant"} (forall idx$: int :: 
-    (0 <= idx$) && (idx$ < (R[Net#c] + C[Net#c])) ==> (M[Net#c][idx$] == M[Net#a][idx$])
+  assume (forall idx$: int :: 
+    (0 <= idx$) && (idx$ < C[Net#e]) ==> (M[Net#e][idx$] == M[Net#c][idx$])
   );
-  assert {:msg "  The network might not preserve the channel invariant"} (forall idx$: int :: 
-    (0 <= idx$) && (idx$ < (R[Net#d] + C[Net#d])) ==> (M[Net#d][idx$] == M[Net#b][idx$])
+  assume (forall idx$: int :: 
+    (0 <= idx$) && (idx$ < C[Net#a]) ==> (SqnCh[Net#a][idx$] == idx$)
   );
-  assert {:msg "  The network might not preserve the channel invariant"} (forall idx$: int :: 
-    (0 <= idx$) && (idx$ < (R[Net#e] + C[Net#e])) ==> (M[Net#e][idx$] == M[Net#c][idx$])
+}
+procedure Net#anon$3#input#in#15()
+  modifies C, R, M, I, St, SqnCh, SqnAct;
+{
+  assume 0 <= I[Net#a];
+  assume I[Net#a] <= R[Net#a];
+  assume R[Net#a] <= C[Net#a];
+  assume 0 <= I[Net#b];
+  assume I[Net#b] <= R[Net#b];
+  assume R[Net#b] <= C[Net#b];
+  assume 0 <= I[Net#c];
+  assume I[Net#c] <= R[Net#c];
+  assume R[Net#c] <= C[Net#c];
+  assume 0 <= I[Net#d];
+  assume I[Net#d] <= R[Net#d];
+  assume R[Net#d] <= C[Net#d];
+  assume 0 <= I[Net#e];
+  assume I[Net#e] <= R[Net#e];
+  assume R[Net#e] <= C[Net#e];
+  assume 0 <= I[Net#f];
+  assume I[Net#f] <= R[Net#f];
+  assume R[Net#f] <= C[Net#f];
+  assume 0 <= I[Net#g];
+  assume I[Net#g] <= R[Net#g];
+  assume R[Net#g] <= C[Net#g];
+  assume I[Net#g] == R[Net#g];
+  assume C[Net#a] < 1;
+  assume SqnAct[Net#spl] == R[Net#a];
+  assume SqnAct[Net#pri] == R[Net#b];
+  assume SqnAct[Net#sec] == R[Net#c];
+  assume SqnAct[Net#adj] == R[Net#e];
+  assume (forall i: int :: 
+    (0 <= i) && (i < C[Net#a]) ==> (SqnCh[Net#a][i] == i)
   );
-  assert {:msg "  The network might not preserve the channel invariant"} (forall idx$: int :: 
-    (0 <= idx$) && (idx$ < (R[Net#a] + C[Net#a])) ==> (SqnCh[Net#a][idx$] == idx$)
+  assume (forall i: int :: 
+    (0 <= i) && (i < C[Net#b]) ==> (SqnCh[Net#b][i] == i)
   );
-  assert {:msg "  40.15: The network might not preserve the channel invariant"} SqnAct[Net#spl] == R[Net#a];
-  assert {:msg "  41.15: The network might not preserve the channel invariant"} SqnAct[Net#pri] == R[Net#b];
-  assert {:msg "  42.15: The network might not preserve the channel invariant"} SqnAct[Net#sec] == R[Net#c];
-  assert {:msg "  43.15: The network might not preserve the channel invariant"} SqnAct[Net#adj] == R[Net#e];
-  assert {:msg "  45.16: The network might not preserve the channel invariant"} (forall i: int :: 
-    (0 <= i) && (i < (R[Net#a] + C[Net#a])) ==> (SqnCh[Net#a][i] == i)
+  assume (forall i: int :: 
+    (0 <= i) && (i < C[Net#c]) ==> (SqnCh[Net#c][i] == i)
   );
-  assert {:msg "  46.16: The network might not preserve the channel invariant"} (forall i: int :: 
-    (0 <= i) && (i < (R[Net#b] + C[Net#b])) ==> (SqnCh[Net#b][i] == i)
+  assume (forall i: int :: 
+    (0 <= i) && (i < C[Net#d]) ==> (SqnCh[Net#d][i] == i)
   );
-  assert {:msg "  47.16: The network might not preserve the channel invariant"} (forall i: int :: 
-    (0 <= i) && (i < (R[Net#c] + C[Net#c])) ==> (SqnCh[Net#c][i] == i)
+  assume (forall i: int :: 
+    (0 <= i) && (i < C[Net#e]) ==> (SqnCh[Net#e][i] == i)
   );
-  assert {:msg "  48.16: The network might not preserve the channel invariant"} (forall i: int :: 
-    (0 <= i) && (i < (R[Net#d] + C[Net#d])) ==> (SqnCh[Net#d][i] == i)
+  assume (forall i: int :: 
+    (0 <= i) && (i < C[Net#g]) ==> (SqnCh[Net#g][i] == i)
   );
-  assert {:msg "  49.16: The network might not preserve the channel invariant"} (forall i: int :: 
-    (0 <= i) && (i < (R[Net#e] + C[Net#e])) ==> (SqnCh[Net#e][i] == i)
+  assume (C[Net#f] - R[Net#f]) == 1;
+  assume C[Net#g] == R[Net#e];
+  assume R[Net#e] == M[Net#f][R[Net#f]];
+  assume (forall i: int :: 
+    (0 <= i) && (i < C[Net#g]) ==> (SqnCh[Net#g][i] == i)
   );
-  assert {:msg "  50.16: The network might not preserve the channel invariant"} (forall i: int :: 
-    (0 <= i) && (i < (R[Net#g] + C[Net#g])) ==> (SqnCh[Net#g][i] == i)
-  );
-  assert {:msg "  52.15: The network might not preserve the channel invariant"} C[Net#f] == 1;
-  assert {:msg "  53.15: The network might not preserve the channel invariant"} (R[Net#g] + C[Net#g]) == R[Net#e];
-  assert {:msg "  54.15: The network might not preserve the channel invariant"} R[Net#e] == M[Net#f][R[Net#f]];
-  assert {:msg "  55.16: The network might not preserve the channel invariant"} (forall i: int :: 
-    (0 <= i) && (i < (R[Net#g] + C[Net#g])) ==> (SqnCh[Net#g][i] == i)
-  );
-  if ((0 < R[Net#d]) && (0 < R[Net#e])) {
-    assert {:msg "  57.42: The network might not preserve the channel invariant"} M[Net#d][R[Net#d] - 1] <= M[Net#e][R[Net#e] - 1];
-  }
-  assert {:msg "  58.16: The network might not preserve the channel invariant"} (forall i: int :: 
+  assume (forall i: int :: 
     (0 <= i) && (i < R[Net#e]) ==> (M[Net#g][i] == M[Net#e][i])
   );
+  assume R[Net#a] == C[Net#b];
+  assume R[Net#a] == C[Net#c];
+  assume R[Net#b] == C[Net#d];
+  assume R[Net#c] == C[Net#e];
+  assume (forall idx$: int :: 
+    (0 <= idx$) && (idx$ < C[Net#b]) ==> (M[Net#b][idx$] == M[Net#a][idx$])
+  );
+  assume (forall idx$: int :: 
+    (0 <= idx$) && (idx$ < C[Net#c]) ==> (M[Net#c][idx$] == M[Net#a][idx$])
+  );
+  assume (forall idx$: int :: 
+    (0 <= idx$) && (idx$ < C[Net#d]) ==> (M[Net#d][idx$] == M[Net#b][idx$])
+  );
+  assume (forall idx$: int :: 
+    (0 <= idx$) && (idx$ < C[Net#e]) ==> (M[Net#e][idx$] == M[Net#c][idx$])
+  );
+  assume (forall idx$: int :: 
+    (0 <= idx$) && (idx$ < C[Net#a]) ==> (SqnCh[Net#a][idx$] == idx$)
+  );
+  C[Net#a] := C[Net#a] + 1;
+  assume (forall i: int :: 
+    (0 <= i) && (i < C[Net#a]) ==> (SqnCh[Net#a][i] == i)
+  );
+  assert {:msg "41.15: Channel invariant might be falsified by network input"} SqnAct[Net#spl] == R[Net#a];
+  assert {:msg "42.15: Channel invariant might be falsified by network input"} SqnAct[Net#pri] == R[Net#b];
+  assert {:msg "43.15: Channel invariant might be falsified by network input"} SqnAct[Net#sec] == R[Net#c];
+  assert {:msg "44.15: Channel invariant might be falsified by network input"} SqnAct[Net#adj] == R[Net#e];
+  assert {:msg "46.16: Channel invariant might be falsified by network input"} (forall i: int :: 
+    (0 <= i) && (i < C[Net#a]) ==> (SqnCh[Net#a][i] == i)
+  );
+  assert {:msg "47.16: Channel invariant might be falsified by network input"} (forall i: int :: 
+    (0 <= i) && (i < C[Net#b]) ==> (SqnCh[Net#b][i] == i)
+  );
+  assert {:msg "48.16: Channel invariant might be falsified by network input"} (forall i: int :: 
+    (0 <= i) && (i < C[Net#c]) ==> (SqnCh[Net#c][i] == i)
+  );
+  assert {:msg "49.16: Channel invariant might be falsified by network input"} (forall i: int :: 
+    (0 <= i) && (i < C[Net#d]) ==> (SqnCh[Net#d][i] == i)
+  );
+  assert {:msg "50.16: Channel invariant might be falsified by network input"} (forall i: int :: 
+    (0 <= i) && (i < C[Net#e]) ==> (SqnCh[Net#e][i] == i)
+  );
+  assert {:msg "51.16: Channel invariant might be falsified by network input"} (forall i: int :: 
+    (0 <= i) && (i < C[Net#g]) ==> (SqnCh[Net#g][i] == i)
+  );
+  assert {:msg "53.15: Channel invariant might be falsified by network input"} (C[Net#f] - R[Net#f]) == 1;
+  assert {:msg "54.15: Channel invariant might be falsified by network input"} C[Net#g] == R[Net#e];
+  assert {:msg "55.15: Channel invariant might be falsified by network input"} R[Net#e] == M[Net#f][R[Net#f]];
+  assert {:msg "56.16: Channel invariant might be falsified by network input"} (forall i: int :: 
+    (0 <= i) && (i < C[Net#g]) ==> (SqnCh[Net#g][i] == i)
+  );
+  assert {:msg "59.16: Channel invariant might be falsified by network input"} (forall i: int :: 
+    (0 <= i) && (i < R[Net#e]) ==> (M[Net#g][i] == M[Net#e][i])
+  );
+  assert {:msg "Channel invariant might be falsified by network input"} R[Net#a] == C[Net#b];
+  assert {:msg "Channel invariant might be falsified by network input"} R[Net#a] == C[Net#c];
+  assert {:msg "Channel invariant might be falsified by network input"} R[Net#b] == C[Net#d];
+  assert {:msg "Channel invariant might be falsified by network input"} R[Net#c] == C[Net#e];
+  assert {:msg "Channel invariant might be falsified by network input"} (forall idx$: int :: 
+    (0 <= idx$) && (idx$ < C[Net#b]) ==> (M[Net#b][idx$] == M[Net#a][idx$])
+  );
+  assert {:msg "Channel invariant might be falsified by network input"} (forall idx$: int :: 
+    (0 <= idx$) && (idx$ < C[Net#c]) ==> (M[Net#c][idx$] == M[Net#a][idx$])
+  );
+  assert {:msg "Channel invariant might be falsified by network input"} (forall idx$: int :: 
+    (0 <= idx$) && (idx$ < C[Net#d]) ==> (M[Net#d][idx$] == M[Net#b][idx$])
+  );
+  assert {:msg "Channel invariant might be falsified by network input"} (forall idx$: int :: 
+    (0 <= idx$) && (idx$ < C[Net#e]) ==> (M[Net#e][idx$] == M[Net#c][idx$])
+  );
+  assert {:msg "Channel invariant might be falsified by network input"} (forall idx$: int :: 
+    (0 <= idx$) && (idx$ < C[Net#a]) ==> (SqnCh[Net#a][idx$] == idx$)
+  );
+}
+procedure Net#anon$3#exit#16()
+  modifies C, R, M, I, St, SqnCh, SqnAct;
+{
+  assume 0 <= I[Net#a];
+  assume I[Net#a] <= R[Net#a];
+  assume R[Net#a] <= C[Net#a];
+  assume 0 <= I[Net#b];
+  assume I[Net#b] <= R[Net#b];
+  assume R[Net#b] <= C[Net#b];
+  assume 0 <= I[Net#c];
+  assume I[Net#c] <= R[Net#c];
+  assume R[Net#c] <= C[Net#c];
+  assume 0 <= I[Net#d];
+  assume I[Net#d] <= R[Net#d];
+  assume R[Net#d] <= C[Net#d];
+  assume 0 <= I[Net#e];
+  assume I[Net#e] <= R[Net#e];
+  assume R[Net#e] <= C[Net#e];
+  assume 0 <= I[Net#f];
+  assume I[Net#f] <= R[Net#f];
+  assume R[Net#f] <= C[Net#f];
+  assume 0 <= I[Net#g];
+  assume I[Net#g] <= R[Net#g];
+  assume R[Net#g] <= C[Net#g];
+  assume I[Net#g] == R[Net#g];
+  assume SqnAct[Net#spl] == R[Net#a];
+  assume SqnAct[Net#pri] == R[Net#b];
+  assume SqnAct[Net#sec] == R[Net#c];
+  assume SqnAct[Net#adj] == R[Net#e];
+  assume (forall i: int :: 
+    (0 <= i) && (i < C[Net#a]) ==> (SqnCh[Net#a][i] == i)
+  );
+  assume (forall i: int :: 
+    (0 <= i) && (i < C[Net#b]) ==> (SqnCh[Net#b][i] == i)
+  );
+  assume (forall i: int :: 
+    (0 <= i) && (i < C[Net#c]) ==> (SqnCh[Net#c][i] == i)
+  );
+  assume (forall i: int :: 
+    (0 <= i) && (i < C[Net#d]) ==> (SqnCh[Net#d][i] == i)
+  );
+  assume (forall i: int :: 
+    (0 <= i) && (i < C[Net#e]) ==> (SqnCh[Net#e][i] == i)
+  );
+  assume (forall i: int :: 
+    (0 <= i) && (i < C[Net#g]) ==> (SqnCh[Net#g][i] == i)
+  );
+  assume (C[Net#f] - R[Net#f]) == 1;
+  assume C[Net#g] == R[Net#e];
+  assume R[Net#e] == M[Net#f][R[Net#f]];
+  assume (forall i: int :: 
+    (0 <= i) && (i < C[Net#g]) ==> (SqnCh[Net#g][i] == i)
+  );
+  assume (forall i: int :: 
+    (0 <= i) && (i < R[Net#e]) ==> (M[Net#g][i] == M[Net#e][i])
+  );
+  assume R[Net#a] == C[Net#b];
+  assume R[Net#a] == C[Net#c];
+  assume R[Net#b] == C[Net#d];
+  assume R[Net#c] == C[Net#e];
+  assume (forall idx$: int :: 
+    (0 <= idx$) && (idx$ < C[Net#b]) ==> (M[Net#b][idx$] == M[Net#a][idx$])
+  );
+  assume (forall idx$: int :: 
+    (0 <= idx$) && (idx$ < C[Net#c]) ==> (M[Net#c][idx$] == M[Net#a][idx$])
+  );
+  assume (forall idx$: int :: 
+    (0 <= idx$) && (idx$ < C[Net#d]) ==> (M[Net#d][idx$] == M[Net#b][idx$])
+  );
+  assume (forall idx$: int :: 
+    (0 <= idx$) && (idx$ < C[Net#e]) ==> (M[Net#e][idx$] == M[Net#c][idx$])
+  );
+  assume (forall idx$: int :: 
+    (0 <= idx$) && (idx$ < C[Net#a]) ==> (SqnCh[Net#a][idx$] == idx$)
+  );
+  assume (C[Net#a] - I[Net#a]) == 1;
+  assume !(1 <= (C[Net#a] - R[Net#a]));
+  assume !(1 <= (C[Net#b] - R[Net#b]));
+  assume !(1 <= (C[Net#c] - R[Net#c]));
+  assume !((!((1 <= (C[Net#d] - R[Net#d])) && (1 <= (C[Net#f] - R[Net#f])) && (SqnCh[Net#d][R[Net#d] - 0] < M[Net#f][R[Net#f] - 0]))) && (1 <= (C[Net#d] - R[Net#d])) && (1 <= (C[Net#e] - R[Net#e])) && (1 <= (C[Net#f] - R[Net#f])) && (SqnCh[Net#d][R[Net#d] - 0] == SqnCh[Net#e][R[Net#e] - 0]) && (SqnCh[Net#d][R[Net#d] - 0] == M[Net#f][R[Net#f] - 0]));
+  assume !((!((1 <= (C[Net#d] - R[Net#d])) && (1 <= (C[Net#f] - R[Net#f])) && (SqnCh[Net#d][R[Net#d] - 0] < M[Net#f][R[Net#f] - 0]))) && (!((1 <= (C[Net#d] - R[Net#d])) && (1 <= (C[Net#e] - R[Net#e])) && (1 <= (C[Net#f] - R[Net#f])) && (SqnCh[Net#d][R[Net#d] - 0] == SqnCh[Net#e][R[Net#e] - 0]) && (SqnCh[Net#d][R[Net#d] - 0] == M[Net#f][R[Net#f] - 0]))) && (1 <= (C[Net#e] - R[Net#e])) && (1 <= (C[Net#f] - R[Net#f])));
+  assume !((1 <= (C[Net#d] - R[Net#d])) && (1 <= (C[Net#f] - R[Net#f])) && (SqnCh[Net#d][R[Net#d] - 0] < M[Net#f][R[Net#f] - 0]));
+  assert {:msg "34.14: Network action postcondition might not hold"} (forall i: int :: 
+    (0 <= i) && (i < C[Net#g]) ==> (SqnCh[Net#g][i] == i)
+  );
+  assert {:msg "35.14: Network action postcondition might not hold"} (forall i: int :: 
+    (0 <= i) && (i < C[Net#g]) ==> (M[Net#g][i] == M[Net#a][i])
+  );
+  R[Net#g] := R[Net#g] + 1;
+  I := R;
+  assert {:msg "41.15: The network might not preserve the channel invariant (#171)"} SqnAct[Net#spl] == R[Net#a];
+  assert {:msg "42.15: The network might not preserve the channel invariant (#172)"} SqnAct[Net#pri] == R[Net#b];
+  assert {:msg "43.15: The network might not preserve the channel invariant (#173)"} SqnAct[Net#sec] == R[Net#c];
+  assert {:msg "44.15: The network might not preserve the channel invariant (#174)"} SqnAct[Net#adj] == R[Net#e];
+  assert {:msg "46.16: The network might not preserve the channel invariant (#175)"} (forall i: int :: 
+    (0 <= i) && (i < C[Net#a]) ==> (SqnCh[Net#a][i] == i)
+  );
+  assert {:msg "47.16: The network might not preserve the channel invariant (#176)"} (forall i: int :: 
+    (0 <= i) && (i < C[Net#b]) ==> (SqnCh[Net#b][i] == i)
+  );
+  assert {:msg "48.16: The network might not preserve the channel invariant (#177)"} (forall i: int :: 
+    (0 <= i) && (i < C[Net#c]) ==> (SqnCh[Net#c][i] == i)
+  );
+  assert {:msg "49.16: The network might not preserve the channel invariant (#178)"} (forall i: int :: 
+    (0 <= i) && (i < C[Net#d]) ==> (SqnCh[Net#d][i] == i)
+  );
+  assert {:msg "50.16: The network might not preserve the channel invariant (#179)"} (forall i: int :: 
+    (0 <= i) && (i < C[Net#e]) ==> (SqnCh[Net#e][i] == i)
+  );
+  assert {:msg "51.16: The network might not preserve the channel invariant (#180)"} (forall i: int :: 
+    (0 <= i) && (i < C[Net#g]) ==> (SqnCh[Net#g][i] == i)
+  );
+  assert {:msg "53.15: The network might not preserve the channel invariant (#181)"} (C[Net#f] - R[Net#f]) == 1;
+  assert {:msg "54.15: The network might not preserve the channel invariant (#182)"} C[Net#g] == R[Net#e];
+  assert {:msg "55.15: The network might not preserve the channel invariant (#183)"} R[Net#e] == M[Net#f][R[Net#f]];
+  assert {:msg "56.16: The network might not preserve the channel invariant (#184)"} (forall i: int :: 
+    (0 <= i) && (i < C[Net#g]) ==> (SqnCh[Net#g][i] == i)
+  );
+  assert {:msg "59.16: The network might not preserve the channel invariant (#185)"} (forall i: int :: 
+    (0 <= i) && (i < R[Net#e]) ==> (M[Net#g][i] == M[Net#e][i])
+  );
+  assert {:msg "The network might not preserve the channel invariant (#186)"} R[Net#a] == C[Net#b];
+  assert {:msg "The network might not preserve the channel invariant (#187)"} R[Net#a] == C[Net#c];
+  assert {:msg "The network might not preserve the channel invariant (#188)"} R[Net#b] == C[Net#d];
+  assert {:msg "The network might not preserve the channel invariant (#189)"} R[Net#c] == C[Net#e];
+  assert {:msg "The network might not preserve the channel invariant (#190)"} (forall idx$: int :: 
+    (0 <= idx$) && (idx$ < C[Net#b]) ==> (M[Net#b][idx$] == M[Net#a][idx$])
+  );
+  assert {:msg "The network might not preserve the channel invariant (#191)"} (forall idx$: int :: 
+    (0 <= idx$) && (idx$ < C[Net#c]) ==> (M[Net#c][idx$] == M[Net#a][idx$])
+  );
+  assert {:msg "The network might not preserve the channel invariant (#192)"} (forall idx$: int :: 
+    (0 <= idx$) && (idx$ < C[Net#d]) ==> (M[Net#d][idx$] == M[Net#b][idx$])
+  );
+  assert {:msg "The network might not preserve the channel invariant (#193)"} (forall idx$: int :: 
+    (0 <= idx$) && (idx$ < C[Net#e]) ==> (M[Net#e][idx$] == M[Net#c][idx$])
+  );
+  assert {:msg "The network might not preserve the channel invariant (#194)"} (forall idx$: int :: 
+    (0 <= idx$) && (idx$ < C[Net#a]) ==> (SqnCh[Net#a][idx$] == idx$)
+  );
   C[Net#f] := C[Net#f] - 1;
-  assert {:msg "  38.13: The network might not preserve the network invariant"} R[Net#e] == M[Net#f][R[Net#f]];
-  assert {:msg "  32.3: The network might leave unread tokens on channel a"} C[Net#a] == 0;
-  assert {:msg "  32.3: The network might leave unread tokens on channel b"} C[Net#b] == 0;
-  assert {:msg "  32.3: The network might leave unread tokens on channel c"} C[Net#c] == 0;
-  assert {:msg "  32.3: The network might leave unread tokens on channel d"} C[Net#d] == 0;
-  assert {:msg "  32.3: The network might leave unread tokens on channel e"} C[Net#e] == 0;
-  assert {:msg "  32.3: The network might leave unread tokens on channel f"} C[Net#f] == 0;
-  assert {:msg "  32.3: The network might not produce the specified number of tokens on output out"} C[Net#g] == 0;
+  assert {:msg "39.13: The network might not preserve the network invariant"} R[Net#e] == M[Net#f][R[Net#f]];
+  assert {:msg "32.3: The network might leave unread tokens on channel a"} C[Net#a] == R[Net#a];
+  assert {:msg "32.3: The network might leave unread tokens on channel b"} C[Net#b] == R[Net#b];
+  assert {:msg "32.3: The network might leave unread tokens on channel c"} C[Net#c] == R[Net#c];
+  assert {:msg "32.3: The network might leave unread tokens on channel d"} C[Net#d] == R[Net#d];
+  assert {:msg "32.3: The network might leave unread tokens on channel e"} C[Net#e] == R[Net#e];
+  assert {:msg "32.3: The network might leave unread tokens on channel f"} C[Net#f] == R[Net#f];
+  assert {:msg "32.3: The network might not produce the specified number of tokens on output out"} C[Net#g] == R[Net#g];
 }
